{
    "processInformation": {
        "dataSetInformation": {
            "UUID": "549f3296-efca-4d5f-ac64-de32f6b3a6f5",
            "name": {
                "baseName": [
                    {
                        "value": "7 Ready-mixed concrete mixtures: Betonpav P30C4D31S5XC2XC1",
                        "lang": "en"
                    }
                ]
            },
            "generalComment": [
                {
                    "value": "1 m3 of ready-mix concrete produced at factory gate\n\nThe study has been carried out based on specific primary data collected directly from the company through the compilation of data collection questionnaires. For all processes for which specific data are not available, reference is made to generic data taken mainly from the LCA database Ecoinvent v3.9.1 or from other verified LCA studies. The generic data used satisfy the data quality characteristics required by the Program Operator Regulations and the reference PCRs and can come from site-specific sources or average data. The use of proxy data is  limited.\n\n\n\n\n\"EN 15804: 2019 allocation rules have been adopted. For virgin raw materials, both the impacts associated with the materials themselves and those associated with the related production processes were considered.\nWith regard to raw materials of recycled origin, only the impacts of the recycling process starting from the End of Waste status are considered. Outputs subject to recycling are considered inputs for the next life cycle; their impacts were assessed up to the End of Waste status.\nSome impacts of the production plant (e.g., electricity, water and diesel consumption) have been allocated among the outputs of the 2022 production based on physical properties.\"\n\n\nThe cut-off rules in EN 15804:2019 have been applied, the applied cut-offs do not exceed 1% of the mass and energy flows entering the system.\n\n\n",
                    "lang": "en"
                }
            ]
        },
        "quantitativeReference": {
            "referenceToReferenceFlow": [
                1
            ],
            "type": "Reference flow(s)"
        },
        "time": {
            "referenceYear": 2024,
            "dataSetValidUntil": 2029,
            "other": {
                "anies": [
                    {
                        "name": "publicationDateOfEPD",
                        "value": 1719360000000
                    }
                ]
            }
        },
        "geography": {
            "locationOfOperationSupplyOrProduction": {
                "descriptionOfRestrictions": [
                    {
                        "value": "Italy\n",
                        "lang": "en"
                    }
                ],
                "location": "IT"
            }
        },
        "technology": {
            "technologicalApplicability": [
                {
                    "value": "\"Multibeton XC concretes are specifically formulated to vary within a broad range, considering factors such as mechanical strength requirements, environmental conditions of the construction site, and casting complexity. They are particularly recommended for constructions where the reinforcement is exposed to air and moisture, thereby posing a risk of carbonation-induced reinforcement bar corrosion. \nDrainbeton is a specialized concrete tailored for drainage and sound absorption, It's the optimal choice for creating permeable pavements.\nBetonpav is optimal for internal and external flooring, in the infrastructural, industrial, residential and tertiary sectors, subjected to the action of static and dynamic loads. Compared to ordinary concrete, it is characterized by faster setting times and an easier installation.\"\n \"Ready mix concrete:\nMultibeton: R30C4D31S4XC2/XC1, R30C3D16SCCXC2/XC1, R30C4D31S5XC2/XC1, R30C4D16S4XC2/XC1, R30C3D31S4XC2/XC1, R40C4D31S4XC4/XC3/XC2/XC1/XA2;\nBetonpav: P30C4D31S5XC2/XC1, P35C4D31S5XC2/XC1, P30C4D31S4XC2/XC1;\nDrainbeton: DB30C4D08S2.\"",
                    "lang": "en"
                }
            ]
        }
    },
    "modellingAndValidation": {
        "LCIMethodAndAllocation": {
            "typeOfDataSet": "EPD",
            "referenceToLCAMethodDetails": [
                {
                    "shortDescription": [
                        {
                            "value": "PCR ICMQ 3.0 - rev. 3.0 - Products and services for construction",
                            "lang": "en"
                        }
                    ],
                    "type": "source data set",
                    "refObjectId": "f6000c03-9880-4cfa-ac2e-20eef15ecaff",
                    "version": "00.00.000"
                }
            ],
            "other": {
                "anies": [
                    {
                        "name": "subType",
                        "value": "specific dataset"
                    }
                ]
            }
        },
        "dataSourcesTreatmentAndRepresentativeness": {
            "referenceToDataSource": [
                {
                    "shortDescription": [
                        {
                            "value": "ecoinvent database (all versions)",
                            "lang": "en"
                        }
                    ],
                    "type": "source data set",
                    "refObjectId": "b497a91f-e14b-4b69-8f28-f50eb1576766",
                    "version": "00.03.001",
                    "uri": "http://openlca.org/ilcd/resource/sources/b497a91f-e14b-4b69-8f28-f50eb1576766"
                }
            ],
            "useAdviceForDataSet": [
                {
                    "value": "cradle to gate with options: A1, A2, A3, C1, C2, C3, C4, D\n",
                    "lang": "en"
                }
            ],
            "other": {
                "anies": [
                    {
                        "name": "referenceToOriginalEPD",
                        "value": {
                            "type": "source data set",
                            "refObjectId": "99cf2db0-655c-4079-9489-2a3fec36a1e6",
                            "version": "00.00.000"
                        }
                    }
                ]
            }
        },
        "validation": {
            "review": [
                {
                    "referenceToNameOfReviewerAndInstitution": [
                        {
                            "shortDescription": [
                                {
                                    "value": "ICMQ spa",
                                    "lang": "en"
                                }
                            ],
                            "type": "contact data set",
                            "refObjectId": "cbb9d118-f872-4b99-920a-b1078fce25da",
                            "version": "00.00.001"
                        }
                    ],
                    "type": "Independent external review"
                }
            ]
        },
        "complianceDeclarations": {
            "compliance": [
                {
                    "referenceToComplianceSystem": {
                        "shortDescription": [
                            {
                                "value": "EN 15804+A2",
                                "lang": "en"
                            }
                        ],
                        "type": "source data set",
                        "refObjectId": "c0016b33-8cf7-415c-ac6e-deba0d21440d",
                        "version": "00.02.000"
                    },
                    "approvalOfOverallCompliance": "Fully compliant",
                    "nomenclatureCompliance": "Fully compliant",
                    "methodologicalCompliance": "Fully compliant",
                    "reviewCompliance": "Fully compliant",
                    "documentationCompliance": "Fully compliant",
                    "qualityCompliance": "Fully compliant"
                },
                {
                    "referenceToComplianceSystem": {
                        "shortDescription": [
                            {
                                "value": "ISO 14025",
                                "lang": "en"
                            }
                        ],
                        "type": "source data set",
                        "refObjectId": "4f2eb655-6e44-4874-a95a-e28f5442cd4d",
                        "version": "00.00.001"
                    },
                    "approvalOfOverallCompliance": "Fully compliant",
                    "nomenclatureCompliance": "Fully compliant",
                    "methodologicalCompliance": "Fully compliant",
                    "reviewCompliance": "Fully compliant",
                    "documentationCompliance": "Fully compliant",
                    "qualityCompliance": "Fully compliant"
                },
                {
                    "referenceToComplianceSystem": {
                        "shortDescription": [
                            {
                                "value": "ISO 21930",
                                "lang": "en"
                            }
                        ],
                        "type": "source data set",
                        "refObjectId": "9c1e8451-2321-4498-b459-b6568b6b6547",
                        "version": "00.00.001"
                    },
                    "approvalOfOverallCompliance": "Fully compliant",
                    "nomenclatureCompliance": "Fully compliant",
                    "methodologicalCompliance": "Fully compliant",
                    "reviewCompliance": "Fully compliant",
                    "documentationCompliance": "Fully compliant",
                    "qualityCompliance": "Fully compliant"
                }
            ]
        }
    },
    "administrativeInformation": {
        "dataGenerator": {
            "referenceToPersonOrEntityGeneratingTheDataSet": [
                {
                    "shortDescription": [
                        {
                            "value": "LCA.no AS",
                            "lang": "en"
                        }
                    ],
                    "type": "contact data set",
                    "refObjectId": "77a6868e-b256-47c8-a410-32706b6e1814",
                    "version": "00.00.001"
                }
            ]
        },
        "dataEntryBy": {
            "timeStamp": 1723217715000,
            "referenceToDataSetFormat": [
                {
                    "shortDescription": [
                        {
                            "value": "ILCD format",
                            "lang": "en"
                        }
                    ],
                    "type": "source data set",
                    "refObjectId": "a97a0155-0234-4b87-b4ce-a45da52f2a40",
                    "version": "01.00.000",
                    "uri": "http://lca.jrc.ec.europa.eu/lcainfohub/sample_data/ilcd/sources/ILCD_Format_a97a0155-0234-4b87-b4ce-a45da52f2a40_01.00.000.xml"
                },
                {
                    "shortDescription": [
                        {
                            "value": "EPD Data Format Extensions v1.2",
                            "lang": "no"
                        },
                        {
                            "value": "EPD Data Format Extensions v1.2",
                            "lang": "en"
                        },
                        {
                            "value": "EPD-Datenformaterweiterungen v1.2",
                            "lang": "de"
                        }
                    ],
                    "type": "source data set",
                    "refObjectId": "a29449fd-aa2f-4de8-b5d7-4b06b43c6fde",
                    "version": "00.01.000"
                }
            ]
        },
        "publicationAndOwnership": {
            "dataSetVersion": "00.03.000",
            "dateOfLastRevision": 1721819517527,
            "referenceToRegistrationAuthority": {
                "shortDescription": [
                    {
                        "value": "EPDItaly",
                        "lang": "en"
                    }
                ],
                "type": "contact data set",
                "refObjectId": "9433b9cf-1d4a-420f-8c09-88d2472225b9",
                "version": "00.00.004"
            },
            "registrationNumber": "EPDITALY0725",
            "referenceToOwnershipOfDataSet": {
                "shortDescription": [
                    {
                        "value": "Betonrossi S.p.A.",
                        "lang": "en"
                    }
                ],
                "type": "contact data set",
                "refObjectId": "119038b4-27fe-47cd-b269-a9bfc4a948f1",
                "version": "00.00.000"
            },
            "copyright": true,
            "licenseType": "Free of charge for all users and uses",
            "accessRestrictions": [
                {
                    "value": "None",
                    "lang": "en"
                }
            ],
            "other": {
                "anies": [
                    {
                        "name": "referenceToPublisher",
                        "value": {
                            "shortDescription": [
                                {
                                    "value": "EPDItaly",
                                    "lang": "en"
                                }
                            ],
                            "type": "contact data set",
                            "refObjectId": "9433b9cf-1d4a-420f-8c09-88d2472225b9",
                            "version": "00.00.004"
                        }
                    }
                ]
            }
        }
    },
    "exchanges": {
        "exchange": [
            {
                "referenceToFlowDataSet": {
                    "shortDescription": [
                        {
                            "value": "7 Ready-mixed concrete mixtures: Betonpav P30C4D31S5XC2XC1",
                            "lang": "en"
                        }
                    ],
                    "type": "flow data set",
                    "refObjectId": "504f91c4-1b42-4df4-9565-53e4c28da04a",
                    "version": "00.01.000"
                },
                "functionType": "General reminder flow",
                "exchangeDirection": "Output",
                "meanAmount": 1.0,
                "resultingAmount": 1.0,
                "minimumAmount": 0.0,
                "maximumAmount": 0.0,
                "uncertaintyDistributionType": "undefined",
                "relativeStandardDeviation95In": 0,
                "dataSourceType": "Primary",
                "dataDerivationTypeStatus": "Measured",
                "dataSetInternalID": 1
            },
            {
                "referenceToFlowDataSet": {
                    "shortDescription": [
                        {
                            "value": "Use of renewable primary energy (PERE)",
                            "lang": "en"
                        },
                        {
                            "value": "Fornybar prim\u00e6renergi brukt som energib\u00e6rer (RPEE)",
                            "lang": "no"
                        }
                    ],
                    "type": "flow data set",
                    "refObjectId": "20f32be5-0398-4288-9b6d-accddd195317",
                    "version": "30.00.000"
                },
                "functionType": "General reminder flow",
                "exchangeDirection": "Input",
                "meanAmount": 0.0,
                "resultingAmount": 0.0,
                "minimumAmount": 0.0,
                "maximumAmount": 0.0,
                "uncertaintyDistributionType": "undefined",
                "relativeStandardDeviation95In": 0,
                "dataSourceType": "Primary",
                "dataDerivationTypeStatus": "Measured",
                "other": {
                    "anies": [
                        {
                            "value": "80.609144275060",
                            "module": "A1"
                        },
                        {
                            "value": "0.479953820527",
                            "module": "A2"
                        },
                        {
                            "value": "0.012027888403",
                            "module": "A3"
                        },
                        {
                            "value": "0.199855572452",
                            "module": "C1"
                        },
                        {
                            "value": "0.420173398708",
                            "module": "C2"
                        },
                        {
                            "value": "4.095485248892",
                            "module": "C3"
                        },
                        {
                            "value": "0.003628347601",
                            "module": "C4"
                        },
                        {
                            "value": "-1.122496368187",
                            "module": "D"
                        },
                        {
                            "name": "referenceToUnitGroupDataSet",
                            "value": {
                                "shortDescription": [
                                    {
                                        "value": "MJ"
                                    }
                                ],
                                "type": "unit group data set",
                                "refObjectId": "93a60a57-a3c8-11da-a746-0800200c9a66",
                                "uri": "../unitgroups/93a60a57-a3c8-11da-a746-0800200c9a66"
                            }
                        }
                    ]
                },
                "dataSetInternalID": 2
            },
            {
                "referenceToFlowDataSet": {
                    "shortDescription": [
                        {
                            "value": "Use of renewable primary energy resources used as raw materials (PERM)",
                            "lang": "en"
                        },
                        {
                            "value": "Fornybar prim\u00e6renergi brukt som energib\u00e6rer (RPEE)",
                            "lang": "no"
                        }
                    ],
                    "type": "flow data set",
                    "refObjectId": "fb3ec0de-548d-4508-aea5-00b73bf6f702",
                    "version": "30.00.000"
                },
                "functionType": "General reminder flow",
                "exchangeDirection": "Input",
                "meanAmount": 0.0,
                "resultingAmount": 0.0,
                "minimumAmount": 0.0,
                "maximumAmount": 0.0,
                "uncertaintyDistributionType": "undefined",
                "relativeStandardDeviation95In": 0,
                "dataSourceType": "Primary",
                "dataDerivationTypeStatus": "Measured",
                "other": {
                    "anies": [
                        {
                            "value": "2.424335417311",
                            "module": "A1"
                        },
                        {
                            "value": "0.074648524068",
                            "module": "A2"
                        },
                        {
                            "value": "0.002551988572",
                            "module": "A3"
                        },
                        {
                            "value": "0.030195318328",
                            "module": "C1"
                        },
                        {
                            "value": "0.065350714681",
                            "module": "C2"
                        },
                        {
                            "value": "1.122409916532",
                            "module": "C3"
                        },
                        {
                            "value": "0.003725279924",
                            "module": "C4"
                        },
                        {
                            "value": "-0.917339328926",
                            "module": "D"
                        },
                        {
                            "name": "referenceToUnitGroupDataSet",
                            "value": {
                                "shortDescription": [
                                    {
                                        "value": "MJ"
                                    }
                                ],
                                "type": "unit group data set",
                                "refObjectId": "93a60a57-a3c8-11da-a746-0800200c9a66",
                                "uri": "../unitgroups/93a60a57-a3c8-11da-a746-0800200c9a66"
                            }
                        }
                    ]
                },
                "dataSetInternalID": 3
            },
            {
                "referenceToFlowDataSet": {
                    "shortDescription": [
                        {
                            "value": "Total use of renewable primary energy resource (PERT)",
                            "lang": "en"
                        },
                        {
                            "value": "Total bruk av fornybar prim\u00e6renergi (TPE)",
                            "lang": "no"
                        }
                    ],
                    "type": "flow data set",
                    "refObjectId": "53f97275-fa8a-4cdd-9024-65936002acd0",
                    "version": "30.00.000"
                },
                "functionType": "General reminder flow",
                "exchangeDirection": "Input",
                "meanAmount": 0.0,
                "resultingAmount": 0.0,
                "minimumAmount": 0.0,
                "maximumAmount": 0.0,
                "uncertaintyDistributionType": "undefined",
                "relativeStandardDeviation95In": 0,
                "dataSourceType": "Primary",
                "dataDerivationTypeStatus": "Measured",
                "other": {
                    "anies": [
                        {
                            "value": "83.033479943652",
                            "module": "A1"
                        },
                        {
                            "value": "0.554602332413",
                            "module": "A2"
                        },
                        {
                            "value": "0.014579876914",
                            "module": "A3"
                        },
                        {
                            "value": "0.230050890780",
                            "module": "C1"
                        },
                        {
                            "value": "0.485524125194",
                            "module": "C2"
                        },
                        {
                            "value": "5.217895049746",
                            "module": "C3"
                        },
                        {
                            "value": "0.007353627477",
                            "module": "C4"
                        },
                        {
                            "value": "-2.039835674230",
                            "module": "D"
                        },
                        {
                            "name": "referenceToUnitGroupDataSet",
                            "value": {
                                "shortDescription": [
                                    {
                                        "value": "MJ"
                                    }
                                ],
                                "type": "unit group data set",
                                "refObjectId": "93a60a57-a3c8-11da-a746-0800200c9a66",
                                "uri": "../unitgroups/93a60a57-a3c8-11da-a746-0800200c9a66"
                            }
                        }
                    ]
                },
                "dataSetInternalID": 4
            },
            {
                "referenceToFlowDataSet": {
                    "shortDescription": [
                        {
                            "value": "Use of non renewable primary energy (PENRE)",
                            "lang": "en"
                        },
                        {
                            "value": "Ikke fornybar prim\u00e6renergi brukt som energib\u00e6rer (NRPE)",
                            "lang": "no"
                        }
                    ],
                    "type": "flow data set",
                    "refObjectId": "ac857178-2b45-46ec-892a-a9a4332f0372",
                    "version": "30.00.000"
                },
                "functionType": "General reminder flow",
                "exchangeDirection": "Input",
                "meanAmount": 0.0,
                "resultingAmount": 0.0,
                "minimumAmount": 0.0,
                "maximumAmount": 0.0,
                "uncertaintyDistributionType": "undefined",
                "relativeStandardDeviation95In": 0,
                "dataSourceType": "Primary",
                "dataDerivationTypeStatus": "Measured",
                "other": {
                    "anies": [
                        {
                            "value": "875.854246419215",
                            "module": "A1"
                        },
                        {
                            "value": "224.309213178829",
                            "module": "A2"
                        },
                        {
                            "value": "2.278229559304",
                            "module": "A3"
                        },
                        {
                            "value": "125.593564338200",
                            "module": "C1"
                        },
                        {
                            "value": "196.370495752903",
                            "module": "C2"
                        },
                        {
                            "value": "89.240818427227",
                            "module": "C3"
                        },
                        {
                            "value": "1.754607829801",
                            "module": "C4"
                        },
                        {
                            "value": "-112.462946864964",
                            "module": "D"
                        },
                        {
                            "name": "referenceToUnitGroupDataSet",
                            "value": {
                                "shortDescription": [
                                    {
                                        "value": "MJ"
                                    }
                                ],
                                "type": "unit group data set",
                                "refObjectId": "93a60a57-a3c8-11da-a746-0800200c9a66",
                                "uri": "../unitgroups/93a60a57-a3c8-11da-a746-0800200c9a66"
                            }
                        }
                    ]
                },
                "dataSetInternalID": 5
            },
            {
                "referenceToFlowDataSet": {
                    "shortDescription": [
                        {
                            "value": "Use of non renewable primary energy resources used as raw materials (PENRM)",
                            "lang": "en"
                        },
                        {
                            "value": "Ikke fornybar prim\u00e6renergi brukt som r\u00e5materiale (NRPM)",
                            "lang": "no"
                        }
                    ],
                    "type": "flow data set",
                    "refObjectId": "1421caa0-679d-4bf4-b282-0eb850ccae27",
                    "version": "30.00.000"
                },
                "functionType": "General reminder flow",
                "exchangeDirection": "Input",
                "meanAmount": 0.0,
                "resultingAmount": 0.0,
                "minimumAmount": 0.0,
                "maximumAmount": 0.0,
                "uncertaintyDistributionType": "undefined",
                "relativeStandardDeviation95In": 0,
                "dataSourceType": "Primary",
                "dataDerivationTypeStatus": "Measured",
                "other": {
                    "anies": [
                        {
                            "value": "0.031385901773",
                            "module": "A1"
                        },
                        {
                            "value": "0.000023001081",
                            "module": "A2"
                        },
                        {
                            "value": "0.000002059840",
                            "module": "A3"
                        },
                        {
                            "value": "0.000332124967",
                            "module": "C1"
                        },
                        {
                            "value": "0.000020136193",
                            "module": "C2"
                        },
                        {
                            "value": "0.000109901316",
                            "module": "C3"
                        },
                        {
                            "value": "0.000005852766",
                            "module": "C4"
                        },
                        {
                            "value": "-0.000298049847",
                            "module": "D"
                        },
                        {
                            "name": "referenceToUnitGroupDataSet",
                            "value": {
                                "shortDescription": [
                                    {
                                        "value": "MJ"
                                    }
                                ],
                                "type": "unit group data set",
                                "refObjectId": "93a60a57-a3c8-11da-a746-0800200c9a66",
                                "uri": "../unitgroups/93a60a57-a3c8-11da-a746-0800200c9a66"
                            }
                        }
                    ]
                },
                "dataSetInternalID": 6
            },
            {
                "referenceToFlowDataSet": {
                    "shortDescription": [
                        {
                            "value": "Total use of non renewable primary energy resource (PENRT)",
                            "lang": "en"
                        },
                        {
                            "value": "Total nicht erneuerbare Prim\u00e4renergie (PENRT)",
                            "lang": "no"
                        }
                    ],
                    "type": "flow data set",
                    "refObjectId": "06159210-646b-4c8d-8583-da9b3b95a6c1",
                    "version": "30.00.000"
                },
                "functionType": "General reminder flow",
                "exchangeDirection": "Input",
                "meanAmount": 0.0,
                "resultingAmount": 0.0,
                "minimumAmount": 0.0,
                "maximumAmount": 0.0,
                "uncertaintyDistributionType": "undefined",
                "relativeStandardDeviation95In": 0,
                "dataSourceType": "Primary",
                "dataDerivationTypeStatus": "Measured",
                "other": {
                    "anies": [
                        {
                            "value": "875.885630815442",
                            "module": "A1"
                        },
                        {
                            "value": "224.309253788234",
                            "module": "A2"
                        },
                        {
                            "value": "2.278231710809",
                            "module": "A3"
                        },
                        {
                            "value": "125.593900822600",
                            "module": "C1"
                        },
                        {
                            "value": "196.370517003267",
                            "module": "C2"
                        },
                        {
                            "value": "89.240929478799",
                            "module": "C3"
                        },
                        {
                            "value": "1.754613681798",
                            "module": "C4"
                        },
                        {
                            "value": "-112.463244339792",
                            "module": "D"
                        },
                        {
                            "name": "referenceToUnitGroupDataSet",
                            "value": {
                                "shortDescription": [
                                    {
                                        "value": "MJ"
                                    }
                                ],
                                "type": "unit group data set",
                                "refObjectId": "93a60a57-a3c8-11da-a746-0800200c9a66",
                                "uri": "../unitgroups/93a60a57-a3c8-11da-a746-0800200c9a66"
                            }
                        }
                    ]
                },
                "dataSetInternalID": 7
            },
            {
                "referenceToFlowDataSet": {
                    "shortDescription": [
                        {
                            "value": "Use of secondary material (SM)",
                            "lang": "en"
                        },
                        {
                            "value": "Bruk av sekund\u00e6re materialer (SM)",
                            "lang": "no"
                        }
                    ],
                    "type": "flow data set",
                    "refObjectId": "c6a1f35f-2d09-4f54-8dfb-97e502e1ce92",
                    "version": "30.00.000"
                },
                "functionType": "General reminder flow",
                "exchangeDirection": "Input",
                "meanAmount": 0.0,
                "resultingAmount": 0.0,
                "minimumAmount": 0.0,
                "maximumAmount": 0.0,
                "uncertaintyDistributionType": "undefined",
                "relativeStandardDeviation95In": 0,
                "dataSourceType": "Primary",
                "dataDerivationTypeStatus": "Measured",
                "other": {
                    "anies": [
                        {
                            "value": "27.885120000000",
                            "module": "A1"
                        },
                        {
                            "value": "0.000000000000",
                            "module": "A2"
                        },
                        {
                            "value": "0.000000000000",
                            "module": "A3"
                        },
                        {
                            "value": "0.000000000000",
                            "module": "C1"
                        },
                        {
                            "value": "0.000000000000",
                            "module": "C2"
                        },
                        {
                            "value": "0.000000000000",
                            "module": "C3"
                        },
                        {
                            "value": "0.000000000000",
                            "module": "C4"
                        },
                        {
                            "value": "0.000000000000",
                            "module": "D"
                        },
                        {
                            "name": "referenceToUnitGroupDataSet",
                            "value": {
                                "shortDescription": [
                                    {
                                        "value": "kg"
                                    }
                                ],
                                "type": "unit group data set",
                                "refObjectId": "ad38d542-3fe9-439d-9b95-2f5f7752acaf",
                                "uri": "../unitgroups/ad38d542-3fe9-439d-9b95-2f5f7752acaf"
                            }
                        }
                    ]
                },
                "dataSetInternalID": 8
            },
            {
                "referenceToFlowDataSet": {
                    "shortDescription": [
                        {
                            "value": "Use of renewable secondary fuels (RSF)",
                            "lang": "en"
                        },
                        {
                            "value": "Bruk av fornybart sekund\u00e6re brensel (RSF)",
                            "lang": "no"
                        }
                    ],
                    "type": "flow data set",
                    "refObjectId": "64333088-a55f-4aa2-9a31-c10b07816787",
                    "version": "30.00.000"
                },
                "functionType": "General reminder flow",
                "exchangeDirection": "Input",
                "meanAmount": 0.0,
                "resultingAmount": 0.0,
                "minimumAmount": 0.0,
                "maximumAmount": 0.0,
                "uncertaintyDistributionType": "undefined",
                "relativeStandardDeviation95In": 0,
                "dataSourceType": "Primary",
                "dataDerivationTypeStatus": "Measured",
                "other": {
                    "anies": [
                        {
                            "value": "240.171840000000",
                            "module": "A1"
                        },
                        {
                            "value": "0.000000000000",
                            "module": "A2"
                        },
                        {
                            "value": "0.000000000000",
                            "module": "A3"
                        },
                        {
                            "value": "0.000000000000",
                            "module": "C1"
                        },
                        {
                            "value": "0.000000000000",
                            "module": "C2"
                        },
                        {
                            "value": "0.000000000000",
                            "module": "C3"
                        },
                        {
                            "value": "0.000000000000",
                            "module": "C4"
                        },
                        {
                            "value": "0.000000000000",
                            "module": "D"
                        },
                        {
                            "name": "referenceToUnitGroupDataSet",
                            "value": {
                                "shortDescription": [
                                    {
                                        "value": "MJ"
                                    }
                                ],
                                "type": "unit group data set",
                                "refObjectId": "93a60a57-a3c8-11da-a746-0800200c9a66",
                                "uri": "../unitgroups/93a60a57-a3c8-11da-a746-0800200c9a66"
                            }
                        }
                    ]
                },
                "dataSetInternalID": 9
            },
            {
                "referenceToFlowDataSet": {
                    "shortDescription": [
                        {
                            "value": "Use of non renewable secondary fuels (NRSF)",
                            "lang": "en"
                        },
                        {
                            "value": "Bruk av ikke fornybart sekund\u00e6re brensel (NRSF)",
                            "lang": "no"
                        }
                    ],
                    "type": "flow data set",
                    "refObjectId": "89def144-d39a-4287-b86f-efde453ddcb2",
                    "version": "30.00.000"
                },
                "functionType": "General reminder flow",
                "exchangeDirection": "Input",
                "meanAmount": 0.0,
                "resultingAmount": 0.0,
                "minimumAmount": 0.0,
                "maximumAmount": 0.0,
                "uncertaintyDistributionType": "undefined",
                "relativeStandardDeviation95In": 0,
                "dataSourceType": "Primary",
                "dataDerivationTypeStatus": "Measured",
                "other": {
                    "anies": [
                        {
                            "value": "670.142400000000",
                            "module": "A1"
                        },
                        {
                            "value": "0.000000000000",
                            "module": "A2"
                        },
                        {
                            "value": "0.000000000000",
                            "module": "A3"
                        },
                        {
                            "value": "0.000000000000",
                            "module": "C1"
                        },
                        {
                            "value": "0.000000000000",
                            "module": "C2"
                        },
                        {
                            "value": "0.000000000000",
                            "module": "C3"
                        },
                        {
                            "value": "0.000000000000",
                            "module": "C4"
                        },
                        {
                            "value": "0.000000000000",
                            "module": "D"
                        },
                        {
                            "name": "referenceToUnitGroupDataSet",
                            "value": {
                                "shortDescription": [
                                    {
                                        "value": "MJ"
                                    }
                                ],
                                "type": "unit group data set",
                                "refObjectId": "93a60a57-a3c8-11da-a746-0800200c9a66",
                                "uri": "../unitgroups/93a60a57-a3c8-11da-a746-0800200c9a66"
                            }
                        }
                    ]
                },
                "dataSetInternalID": 10
            },
            {
                "referenceToFlowDataSet": {
                    "shortDescription": [
                        {
                            "value": "Use of net fresh water (FW)",
                            "lang": "en"
                        },
                        {
                            "value": "Netto bruk av ferskvann (W)",
                            "lang": "no"
                        }
                    ],
                    "type": "flow data set",
                    "refObjectId": "3cf952c8-f3a4-461d-8c96-96456ca62246",
                    "version": "30.00.000"
                },
                "functionType": "General reminder flow",
                "exchangeDirection": "Input",
                "meanAmount": 0.0,
                "resultingAmount": 0.0,
                "minimumAmount": 0.0,
                "maximumAmount": 0.0,
                "uncertaintyDistributionType": "undefined",
                "relativeStandardDeviation95In": 0,
                "dataSourceType": "Primary",
                "dataDerivationTypeStatus": "Measured",
                "other": {
                    "anies": [
                        {
                            "value": "3.199002258849",
                            "module": "A1"
                        },
                        {
                            "value": "0.008821923679",
                            "module": "A2"
                        },
                        {
                            "value": "0.332726383039",
                            "module": "A3"
                        },
                        {
                            "value": "0.005866246267",
                            "module": "C1"
                        },
                        {
                            "value": "0.007723113471",
                            "module": "C2"
                        },
                        {
                            "value": "0.038768425192",
                            "module": "C3"
                        },
                        {
                            "value": "0.000086489197",
                            "module": "C4"
                        },
                        {
                            "value": "-3.212556983062",
                            "module": "D"
                        },
                        {
                            "name": "referenceToUnitGroupDataSet",
                            "value": {
                                "shortDescription": [
                                    {
                                        "value": "m3"
                                    }
                                ],
                                "type": "unit group data set",
                                "refObjectId": "cd950537-0a98-4044-9ba7-9f9a68d0a504",
                                "uri": "../unitgroups/cd950537-0a98-4044-9ba7-9f9a68d0a504"
                            }
                        }
                    ]
                },
                "dataSetInternalID": 11
            },
            {
                "referenceToFlowDataSet": {
                    "shortDescription": [
                        {
                            "value": "Hazardous waste disposed (HWD)",
                            "lang": "en"
                        },
                        {
                            "value": "Avhendet farlig avfall (HW)",
                            "lang": "no"
                        }
                    ],
                    "type": "flow data set",
                    "refObjectId": "430f9e0f-59b2-46a0-8e0d-55e0e84948fc",
                    "version": "30.00.000"
                },
                "functionType": "General reminder flow",
                "exchangeDirection": "Output",
                "meanAmount": 0.0,
                "resultingAmount": 0.0,
                "minimumAmount": 0.0,
                "maximumAmount": 0.0,
                "uncertaintyDistributionType": "undefined",
                "relativeStandardDeviation95In": 0,
                "dataSourceType": "Primary",
                "dataDerivationTypeStatus": "Measured",
                "other": {
                    "anies": [
                        {
                            "value": "0.600230194449",
                            "module": "A1"
                        },
                        {
                            "value": "0.001392701882",
                            "module": "A2"
                        },
                        {
                            "value": "0.000013533591",
                            "module": "A3"
                        },
                        {
                            "value": "0.000789171421",
                            "module": "C1"
                        },
                        {
                            "value": "0.001219234587",
                            "module": "C2"
                        },
                        {
                            "value": "0.000294202728",
                            "module": "C3"
                        },
                        {
                            "value": "0.000010631491",
                            "module": "C4"
                        },
                        {
                            "value": "-0.000474882065",
                            "module": "D"
                        },
                        {
                            "name": "referenceToUnitGroupDataSet",
                            "value": {
                                "shortDescription": [
                                    {
                                        "value": "kg"
                                    }
                                ],
                                "type": "unit group data set",
                                "refObjectId": "ad38d542-3fe9-439d-9b95-2f5f7752acaf",
                                "uri": "../unitgroups/ad38d542-3fe9-439d-9b95-2f5f7752acaf"
                            }
                        }
                    ]
                },
                "dataSetInternalID": 12
            },
            {
                "referenceToFlowDataSet": {
                    "shortDescription": [
                        {
                            "value": "Non hazardous waste dispose (NHWD)",
                            "lang": "en"
                        },
                        {
                            "value": "Avhendet ikke-farlig avfall (NHW)",
                            "lang": "no"
                        }
                    ],
                    "type": "flow data set",
                    "refObjectId": "b29ef66b-e286-4afa-949f-62f1a7b4d7fa",
                    "version": "30.00.000"
                },
                "functionType": "General reminder flow",
                "exchangeDirection": "Output",
                "meanAmount": 0.0,
                "resultingAmount": 0.0,
                "minimumAmount": 0.0,
                "maximumAmount": 0.0,
                "uncertaintyDistributionType": "undefined",
                "relativeStandardDeviation95In": 0,
                "dataSourceType": "Primary",
                "dataDerivationTypeStatus": "Measured",
                "other": {
                    "anies": [
                        {
                            "value": "7.405206075535",
                            "module": "A1"
                        },
                        {
                            "value": "0.010286642360",
                            "module": "A2"
                        },
                        {
                            "value": "29.306287247615",
                            "module": "A3"
                        },
                        {
                            "value": "0.008713309755",
                            "module": "C1"
                        },
                        {
                            "value": "0.009005394702",
                            "module": "C2"
                        },
                        {
                            "value": "0.038791565563",
                            "module": "C3"
                        },
                        {
                            "value": "95.107103902767",
                            "module": "C4"
                        },
                        {
                            "value": "-0.068945631115",
                            "module": "D"
                        },
                        {
                            "name": "referenceToUnitGroupDataSet",
                            "value": {
                                "shortDescription": [
                                    {
                                        "value": "kg"
                                    }
                                ],
                                "type": "unit group data set",
                                "refObjectId": "ad38d542-3fe9-439d-9b95-2f5f7752acaf",
                                "uri": "../unitgroups/ad38d542-3fe9-439d-9b95-2f5f7752acaf"
                            }
                        }
                    ]
                },
                "dataSetInternalID": 13
            },
            {
                "referenceToFlowDataSet": {
                    "shortDescription": [
                        {
                            "value": "Radioactive waste disposed (RWD)",
                            "lang": "en"
                        },
                        {
                            "value": "Avhendet radioaktivt avfall (RW)",
                            "lang": "no"
                        }
                    ],
                    "type": "flow data set",
                    "refObjectId": "3449546e-52ad-4b39-b809-9fb77cea8ff6",
                    "version": "30.00.000"
                },
                "functionType": "General reminder flow",
                "exchangeDirection": "Output",
                "meanAmount": 0.0,
                "resultingAmount": 0.0,
                "minimumAmount": 0.0,
                "maximumAmount": 0.0,
                "uncertaintyDistributionType": "undefined",
                "relativeStandardDeviation95In": 0,
                "dataSourceType": "Primary",
                "dataDerivationTypeStatus": "Measured",
                "other": {
                    "anies": [
                        {
                            "value": "0.000147369655",
                            "module": "A1"
                        },
                        {
                            "value": "0.000018090234",
                            "module": "A2"
                        },
                        {
                            "value": "0.000000498457",
                            "module": "A3"
                        },
                        {
                            "value": "0.000005753634",
                            "module": "C1"
                        },
                        {
                            "value": "0.000015837014",
                            "module": "C2"
                        },
                        {
                            "value": "0.000116926167",
                            "module": "C3"
                        },
                        {
                            "value": "0.000000097879",
                            "module": "C4"
                        },
                        {
                            "value": "-0.000092745997",
                            "module": "D"
                        },
                        {
                            "name": "referenceToUnitGroupDataSet",
                            "value": {
                                "shortDescription": [
                                    {
                                        "value": "kg"
                                    }
                                ],
                                "type": "unit group data set",
                                "refObjectId": "ad38d542-3fe9-439d-9b95-2f5f7752acaf",
                                "uri": "../unitgroups/ad38d542-3fe9-439d-9b95-2f5f7752acaf"
                            }
                        }
                    ]
                },
                "dataSetInternalID": 14
            },
            {
                "referenceToFlowDataSet": {
                    "shortDescription": [
                        {
                            "value": "Components for re-use (CRU)",
                            "lang": "en"
                        },
                        {
                            "value": "Komponenter for gjenbruk (CR)",
                            "lang": "no"
                        }
                    ],
                    "type": "flow data set",
                    "refObjectId": "a2b32f97-3fc7-4af2-b209-525bc6426f33",
                    "version": "30.00.000"
                },
                "functionType": "General reminder flow",
                "exchangeDirection": "Output",
                "meanAmount": 0.0,
                "resultingAmount": 0.0,
                "minimumAmount": 0.0,
                "maximumAmount": 0.0,
                "uncertaintyDistributionType": "undefined",
                "relativeStandardDeviation95In": 0,
                "dataSourceType": "Primary",
                "dataDerivationTypeStatus": "Measured",
                "other": {
                    "anies": [
                        {
                            "value": "0.000000000000",
                            "module": "A1"
                        },
                        {
                            "value": "0.000000000000",
                            "module": "A2"
                        },
                        {
                            "value": "0.000000000000",
                            "module": "A3"
                        },
                        {
                            "value": "0.000000000000",
                            "module": "C1"
                        },
                        {
                            "value": "0.000000000000",
                            "module": "C2"
                        },
                        {
                            "value": "0.000000000000",
                            "module": "C3"
                        },
                        {
                            "value": "0.000000000000",
                            "module": "C4"
                        },
                        {
                            "value": "0.000000000000",
                            "module": "D"
                        },
                        {
                            "name": "referenceToUnitGroupDataSet",
                            "value": {
                                "shortDescription": [
                                    {
                                        "value": "kg"
                                    }
                                ],
                                "type": "unit group data set",
                                "refObjectId": "ad38d542-3fe9-439d-9b95-2f5f7752acaf",
                                "uri": "../unitgroups/ad38d542-3fe9-439d-9b95-2f5f7752acaf"
                            }
                        }
                    ]
                },
                "dataSetInternalID": 15
            },
            {
                "referenceToFlowDataSet": {
                    "shortDescription": [
                        {
                            "value": "Materials for recycling (MFR)",
                            "lang": "en"
                        },
                        {
                            "value": "Materialer for resirkulering (MR)",
                            "lang": "no"
                        }
                    ],
                    "type": "flow data set",
                    "refObjectId": "d7fe48a5-4103-49c8-9aae-b0b5dfdbd6ae",
                    "version": "30.00.000"
                },
                "functionType": "General reminder flow",
                "exchangeDirection": "Output",
                "meanAmount": 0.0,
                "resultingAmount": 0.0,
                "minimumAmount": 0.0,
                "maximumAmount": 0.0,
                "uncertaintyDistributionType": "undefined",
                "relativeStandardDeviation95In": 0,
                "dataSourceType": "Primary",
                "dataDerivationTypeStatus": "Measured",
                "other": {
                    "anies": [
                        {
                            "value": "0.209888000000",
                            "module": "A1"
                        },
                        {
                            "value": "0.000000000000",
                            "module": "A2"
                        },
                        {
                            "value": "4.290000000000",
                            "module": "A3"
                        },
                        {
                            "value": "0.000000000000",
                            "module": "C1"
                        },
                        {
                            "value": "0.000000000000",
                            "module": "C2"
                        },
                        {
                            "value": "2313.574405901171",
                            "module": "C3"
                        },
                        {
                            "value": "0.000000000000",
                            "module": "C4"
                        },
                        {
                            "value": "0.000000000000",
                            "module": "D"
                        },
                        {
                            "name": "referenceToUnitGroupDataSet",
                            "value": {
                                "shortDescription": [
                                    {
                                        "value": "kg"
                                    }
                                ],
                                "type": "unit group data set",
                                "refObjectId": "ad38d542-3fe9-439d-9b95-2f5f7752acaf",
                                "uri": "../unitgroups/ad38d542-3fe9-439d-9b95-2f5f7752acaf"
                            }
                        }
                    ]
                },
                "dataSetInternalID": 16
            },
            {
                "referenceToFlowDataSet": {
                    "shortDescription": [
                        {
                            "value": "Materials for energy recovery (MER)",
                            "lang": "en"
                        },
                        {
                            "value": "Materialer for energigjenvinning (MER)",
                            "lang": "no"
                        }
                    ],
                    "type": "flow data set",
                    "refObjectId": "59a9181c-3aaf-46ee-8b13-2b3723b6e447",
                    "version": "30.00.000"
                },
                "functionType": "General reminder flow",
                "exchangeDirection": "Output",
                "meanAmount": 0.0,
                "resultingAmount": 0.0,
                "minimumAmount": 0.0,
                "maximumAmount": 0.0,
                "uncertaintyDistributionType": "undefined",
                "relativeStandardDeviation95In": 0,
                "dataSourceType": "Primary",
                "dataDerivationTypeStatus": "Measured",
                "other": {
                    "anies": [
                        {
                            "value": "0.000000000000",
                            "module": "A1"
                        },
                        {
                            "value": "0.000000000000",
                            "module": "A2"
                        },
                        {
                            "value": "0.000000000000",
                            "module": "A3"
                        },
                        {
                            "value": "0.000000000000",
                            "module": "C1"
                        },
                        {
                            "value": "0.000000000000",
                            "module": "C2"
                        },
                        {
                            "value": "0.000000000000",
                            "module": "C3"
                        },
                        {
                            "value": "0.000000000000",
                            "module": "C4"
                        },
                        {
                            "value": "0.000000000000",
                            "module": "D"
                        },
                        {
                            "name": "referenceToUnitGroupDataSet",
                            "value": {
                                "shortDescription": [
                                    {
                                        "value": "kg"
                                    }
                                ],
                                "type": "unit group data set",
                                "refObjectId": "ad38d542-3fe9-439d-9b95-2f5f7752acaf",
                                "uri": "../unitgroups/ad38d542-3fe9-439d-9b95-2f5f7752acaf"
                            }
                        }
                    ]
                },
                "dataSetInternalID": 17
            },
            {
                "referenceToFlowDataSet": {
                    "shortDescription": [
                        {
                            "value": "Exported electrical energy (EEE)",
                            "lang": "en"
                        },
                        {
                            "value": "Eksportert elektrisk energi(EEE)",
                            "lang": "no"
                        }
                    ],
                    "type": "flow data set",
                    "refObjectId": "4da0c987-2b76-40d6-9e9e-82a017aaaf29",
                    "version": "30.00.000"
                },
                "functionType": "General reminder flow",
                "exchangeDirection": "Output",
                "meanAmount": 0.0,
                "resultingAmount": 0.0,
                "minimumAmount": 0.0,
                "maximumAmount": 0.0,
                "uncertaintyDistributionType": "undefined",
                "relativeStandardDeviation95In": 0,
                "dataSourceType": "Primary",
                "dataDerivationTypeStatus": "Measured",
                "other": {
                    "anies": [
                        {
                            "value": "0.107942400000",
                            "module": "A1"
                        },
                        {
                            "value": "0.000000000000",
                            "module": "A2"
                        },
                        {
                            "value": "0.000000000000",
                            "module": "A3"
                        },
                        {
                            "value": "0.000000000000",
                            "module": "C1"
                        },
                        {
                            "value": "0.000000000000",
                            "module": "C2"
                        },
                        {
                            "value": "0.000000000000",
                            "module": "C3"
                        },
                        {
                            "value": "0.000000000000",
                            "module": "C4"
                        },
                        {
                            "value": "0.000000000000",
                            "module": "D"
                        },
                        {
                            "name": "referenceToUnitGroupDataSet",
                            "value": {
                                "shortDescription": [
                                    {
                                        "value": "MJ"
                                    }
                                ],
                                "type": "unit group data set",
                                "refObjectId": "93a60a57-a3c8-11da-a746-0800200c9a66",
                                "uri": "../unitgroups/93a60a57-a3c8-11da-a746-0800200c9a66"
                            }
                        }
                    ]
                },
                "dataSetInternalID": 18
            },
            {
                "referenceToFlowDataSet": {
                    "shortDescription": [
                        {
                            "value": "Exported thermal energy (EET)",
                            "lang": "en"
                        },
                        {
                            "value": "Eksportert termisk energi (ETE)",
                            "lang": "no"
                        }
                    ],
                    "type": "flow data set",
                    "refObjectId": "98daf38a-7a79-46d3-9a37-2b7bd0955810",
                    "version": "30.00.000"
                },
                "functionType": "General reminder flow",
                "exchangeDirection": "Output",
                "meanAmount": 0.0,
                "resultingAmount": 0.0,
                "minimumAmount": 0.0,
                "maximumAmount": 0.0,
                "uncertaintyDistributionType": "undefined",
                "relativeStandardDeviation95In": 0,
                "dataSourceType": "Primary",
                "dataDerivationTypeStatus": "Measured",
                "other": {
                    "anies": [
                        {
                            "value": "0.000000000000",
                            "module": "A1"
                        },
                        {
                            "value": "0.000000000000",
                            "module": "A2"
                        },
                        {
                            "value": "0.000000000000",
                            "module": "A3"
                        },
                        {
                            "value": "0.000000000000",
                            "module": "C1"
                        },
                        {
                            "value": "0.000000000000",
                            "module": "C2"
                        },
                        {
                            "value": "0.000000000000",
                            "module": "C3"
                        },
                        {
                            "value": "0.000000000000",
                            "module": "C4"
                        },
                        {
                            "value": "0.000000000000",
                            "module": "D"
                        },
                        {
                            "name": "referenceToUnitGroupDataSet",
                            "value": {
                                "shortDescription": [
                                    {
                                        "value": "MJ"
                                    }
                                ],
                                "type": "unit group data set",
                                "refObjectId": "93a60a57-a3c8-11da-a746-0800200c9a66",
                                "uri": "../unitgroups/93a60a57-a3c8-11da-a746-0800200c9a66"
                            }
                        }
                    ]
                },
                "dataSetInternalID": 19
            }
        ]
    },
    "LCIAResults": {
        "LCIAResult": [
            {
                "referenceToLCIAMethodDataSet": {
                    "shortDescription": [
                        {
                            "value": "Acidification potential, Accumulated Exceedance (AP)",
                            "lang": "en"
                        },
                        {
                            "value": "Forsurningspotensial for kilder p\u00e5 land og vann (AP)",
                            "lang": "no"
                        }
                    ],
                    "type": "LCIA method data set",
                    "refObjectId": "b5c611c6-def3-11e6-bf01-fe55135034f3",
                    "version": "00.01.000"
                },
                "meanAmount": 0.0,
                "uncertaintyDistributionType": "undefined",
                "relativeStandardDeviation95In": 0,
                "other": {
                    "anies": [
                        {
                            "value": "0.247713661316",
                            "module": "A1"
                        },
                        {
                            "value": "0.035242386396",
                            "module": "A2"
                        },
                        {
                            "value": "0.001353732769",
                            "module": "A3"
                        },
                        {
                            "value": "0.085920084155",
                            "module": "C1"
                        },
                        {
                            "value": "0.059603704716",
                            "module": "C2"
                        },
                        {
                            "value": "0.019294199745",
                            "module": "C3"
                        },
                        {
                            "value": "0.001194568652",
                            "module": "C4"
                        },
                        {
                            "value": "-0.044048850638",
                            "module": "D"
                        },
                        {
                            "name": "referenceToUnitGroupDataSet",
                            "value": {
                                "shortDescription": [
                                    {
                                        "value": "mol H+ eqv."
                                    }
                                ],
                                "type": "unit group data set",
                                "refObjectId": "42e089ac-92bf-4bf2-8ca1-5fc40d18f2ed",
                                "uri": "../unitgroups/42e089ac-92bf-4bf2-8ca1-5fc40d18f2ed"
                            }
                        }
                    ]
                }
            },
            {
                "referenceToLCIAMethodDataSet": {
                    "shortDescription": [
                        {
                            "value": "Global Warming Potential - total (GWP-total)",
                            "lang": "en"
                        },
                        {
                            "value": "Globalt oppvarmingspotensial -totalt (GWPtotal)",
                            "lang": "no"
                        }
                    ],
                    "type": "LCIA method data set",
                    "refObjectId": "6a37f984-a4b3-458a-a20a-64418c145fa2",
                    "version": "00.02.000"
                },
                "meanAmount": 0.0,
                "uncertaintyDistributionType": "undefined",
                "relativeStandardDeviation95In": 0,
                "other": {
                    "anies": [
                        {
                            "value": "198.881664740396",
                            "module": "A1"
                        },
                        {
                            "value": "15.695499907432",
                            "module": "A2"
                        },
                        {
                            "value": "0.397280346447",
                            "module": "A3"
                        },
                        {
                            "value": "8.976895700556",
                            "module": "C1"
                        },
                        {
                            "value": "13.889294903362",
                            "module": "C2"
                        },
                        {
                            "value": "5.616133388523",
                            "module": "C3"
                        },
                        {
                            "value": "-1.703506000513",
                            "module": "C4"
                        },
                        {
                            "value": "-7.682181722538",
                            "module": "D"
                        },
                        {
                            "name": "referenceToUnitGroupDataSet",
                            "value": {
                                "shortDescription": [
                                    {
                                        "value": "kg CO2 eqv."
                                    }
                                ],
                                "type": "unit group data set",
                                "refObjectId": "1ebf3012-d0db-4de2-aefd-ef30cedb0be1",
                                "uri": "../unitgroups/1ebf3012-d0db-4de2-aefd-ef30cedb0be1"
                            }
                        }
                    ]
                }
            },
            {
                "referenceToLCIAMethodDataSet": {
                    "shortDescription": [
                        {
                            "value": "Global Warming Potential - biogenic (GWP-biogenic)",
                            "lang": "en"
                        },
                        {
                            "value": "Globalt oppvarmingspotensial - biogene kilder( GWP-biogenic)",
                            "lang": "no"
                        }
                    ],
                    "type": "LCIA method data set",
                    "refObjectId": "2356e1ab-0185-4db5-86e5-16de51c7485c",
                    "version": "00.02.000"
                },
                "meanAmount": 0.0,
                "uncertaintyDistributionType": "undefined",
                "relativeStandardDeviation95In": 0,
                "other": {
                    "anies": [
                        {
                            "value": "1.311785097661",
                            "module": "A1"
                        },
                        {
                            "value": "0.004794213297",
                            "module": "A2"
                        },
                        {
                            "value": "0.000727530369",
                            "module": "A3"
                        },
                        {
                            "value": "0.001669388772",
                            "module": "C1"
                        },
                        {
                            "value": "0.004197072602",
                            "module": "C2"
                        },
                        {
                            "value": "0.084511795994",
                            "module": "C3"
                        },
                        {
                            "value": "-1.832008176577",
                            "module": "C4"
                        },
                        {
                            "value": "-0.111007436854",
                            "module": "D"
                        },
                        {
                            "name": "referenceToUnitGroupDataSet",
                            "value": {
                                "shortDescription": [
                                    {
                                        "value": "kg CO2 eqv."
                                    }
                                ],
                                "type": "unit group data set",
                                "refObjectId": "1ebf3012-d0db-4de2-aefd-ef30cedb0be1",
                                "uri": "../unitgroups/1ebf3012-d0db-4de2-aefd-ef30cedb0be1"
                            }
                        }
                    ]
                }
            },
            {
                "referenceToLCIAMethodDataSet": {
                    "shortDescription": [
                        {
                            "value": "Global Warming Potential - fossil fuels (GWP-fossil)",
                            "lang": "en"
                        },
                        {
                            "value": "Globalt oppvarmingspotensial - fossile brensler (GWP-fossil)",
                            "lang": "no"
                        }
                    ],
                    "type": "LCIA method data set",
                    "refObjectId": "5f635281-343e-44fb-83df-1971b155e6b6",
                    "version": "00.01.000"
                },
                "meanAmount": 0.0,
                "uncertaintyDistributionType": "undefined",
                "relativeStandardDeviation95In": 0,
                "other": {
                    "anies": [
                        {
                            "value": "197.567204227721",
                            "module": "A1"
                        },
                        {
                            "value": "15.690394899195",
                            "module": "A2"
                        },
                        {
                            "value": "0.396543580164",
                            "module": "A3"
                        },
                        {
                            "value": "8.974859475106",
                            "module": "C1"
                        },
                        {
                            "value": "13.884825715592",
                            "module": "C2"
                        },
                        {
                            "value": "5.531382068171",
                            "module": "C3"
                        },
                        {
                            "value": "0.128495725371",
                            "module": "C4"
                        },
                        {
                            "value": "-7.570769848061",
                            "module": "D"
                        },
                        {
                            "name": "referenceToUnitGroupDataSet",
                            "value": {
                                "shortDescription": [
                                    {
                                        "value": "kg CO2 eqv."
                                    }
                                ],
                                "type": "unit group data set",
                                "refObjectId": "1ebf3012-d0db-4de2-aefd-ef30cedb0be1",
                                "uri": "../unitgroups/1ebf3012-d0db-4de2-aefd-ef30cedb0be1"
                            }
                        }
                    ]
                }
            },
            {
                "referenceToLCIAMethodDataSet": {
                    "shortDescription": [
                        {
                            "value": "Global Warming Potential - land use and land use change (GWP-luluc)",
                            "lang": "en"
                        },
                        {
                            "value": "Globalt oppvarmingspotensial arealbruk endringer i bruk av arealer (GWP-luluc)",
                            "lang": "no"
                        }
                    ],
                    "type": "LCIA method data set",
                    "refObjectId": "4331bbdb-978a-490d-8707-eeb047f01a55",
                    "version": "00.02.000"
                },
                "meanAmount": 0.0,
                "uncertaintyDistributionType": "undefined",
                "relativeStandardDeviation95In": 0,
                "other": {
                    "anies": [
                        {
                            "value": "0.017667558201",
                            "module": "A1"
                        },
                        {
                            "value": "0.000310756381",
                            "module": "A2"
                        },
                        {
                            "value": "0.000009235830",
                            "module": "A3"
                        },
                        {
                            "value": "0.000366791787",
                            "module": "C1"
                        },
                        {
                            "value": "0.000272050283",
                            "module": "C2"
                        },
                        {
                            "value": "0.000239409790",
                            "module": "C3"
                        },
                        {
                            "value": "0.000006451256",
                            "module": "C4"
                        },
                        {
                            "value": "-0.000404482748",
                            "module": "D"
                        },
                        {
                            "name": "referenceToUnitGroupDataSet",
                            "value": {
                                "shortDescription": [
                                    {
                                        "value": "kg CO2 eqv."
                                    }
                                ],
                                "type": "unit group data set",
                                "refObjectId": "1ebf3012-d0db-4de2-aefd-ef30cedb0be1",
                                "uri": "../unitgroups/1ebf3012-d0db-4de2-aefd-ef30cedb0be1"
                            }
                        }
                    ]
                }
            },
            {
                "referenceToLCIAMethodDataSet": {
                    "shortDescription": [
                        {
                            "value": "Potential Comparative Toxic Unit for ecosystems (ETP-fw)",
                            "lang": "en"
                        },
                        {
                            "value": "\u00d8kotoksisitet, ferskvann (ETP-fw)",
                            "lang": "no"
                        }
                    ],
                    "type": "LCIA method data set",
                    "refObjectId": "ee1082d1-b0f7-43ca-a1f0-21e2a4a74511",
                    "version": "00.01.000"
                },
                "meanAmount": 0.0,
                "uncertaintyDistributionType": "undefined",
                "relativeStandardDeviation95In": 0,
                "other": {
                    "anies": [
                        {
                            "value": "38.682453737794",
                            "module": "A1"
                        },
                        {
                            "value": "94.585560943150",
                            "module": "A2"
                        },
                        {
                            "value": "1.798428394327",
                            "module": "A3"
                        },
                        {
                            "value": "56.464040857140",
                            "module": "C1"
                        },
                        {
                            "value": "82.218104138259",
                            "module": "C2"
                        },
                        {
                            "value": "9.524185332351",
                            "module": "C3"
                        },
                        {
                            "value": "0.777107653419",
                            "module": "C4"
                        },
                        {
                            "value": "-26.503041578251",
                            "module": "D"
                        },
                        {
                            "name": "referenceToUnitGroupDataSet",
                            "value": {
                                "shortDescription": [
                                    {
                                        "value": "CTUe"
                                    }
                                ],
                                "type": "unit group data set",
                                "refObjectId": "aa959ded-f1eb-4efb-9c5c-2d60be36b3e6",
                                "uri": "../unitgroups/aa959ded-f1eb-4efb-9c5c-2d60be36b3e6"
                            }
                        }
                    ]
                }
            },
            {
                "referenceToLCIAMethodDataSet": {
                    "shortDescription": [
                        {
                            "value": "Potential incidence of disease due to PM emissions (PM)",
                            "lang": "en"
                        },
                        {
                            "value": "Partikkelutslipp (PM)",
                            "lang": "no"
                        }
                    ],
                    "type": "LCIA method data set",
                    "refObjectId": "b5c602c6-def3-11e6-bf01-fe55135034f3",
                    "version": "00.01.000"
                },
                "meanAmount": 0.0,
                "uncertaintyDistributionType": "undefined",
                "relativeStandardDeviation95In": 0,
                "other": {
                    "anies": [
                        {
                            "value": "0.000003873123",
                            "module": "A1"
                        },
                        {
                            "value": "0.000001281212",
                            "module": "A2"
                        },
                        {
                            "value": "0.000000040339",
                            "module": "A3"
                        },
                        {
                            "value": "0.000002423612",
                            "module": "C1"
                        },
                        {
                            "value": "0.000001200304",
                            "module": "C2"
                        },
                        {
                            "value": "0.000017421211",
                            "module": "C3"
                        },
                        {
                            "value": "0.000000033085",
                            "module": "C4"
                        },
                        {
                            "value": "-0.000000929343",
                            "module": "D"
                        },
                        {
                            "name": "referenceToUnitGroupDataSet",
                            "value": {
                                "shortDescription": [
                                    {
                                        "value": "disease incidence"
                                    }
                                ],
                                "type": "unit group data set",
                                "refObjectId": "3883559b-648f-4afc-8ba2-0bd24f3affa3",
                                "uri": "../unitgroups/3883559b-648f-4afc-8ba2-0bd24f3affa3"
                            }
                        }
                    ]
                }
            },
            {
                "referenceToLCIAMethodDataSet": {
                    "shortDescription": [
                        {
                            "value": "Eutrophication potential - marine (EP-marine)",
                            "lang": "en"
                        },
                        {
                            "value": "Overgj\u00f8dslingspotensial til hav (EP-marine), hav og jord",
                            "lang": "no"
                        }
                    ],
                    "type": "LCIA method data set",
                    "refObjectId": "b5c619fa-def3-11e6-bf01-fe55135034f3",
                    "version": "00.01.000"
                },
                "meanAmount": 0.0,
                "uncertaintyDistributionType": "undefined",
                "relativeStandardDeviation95In": 0,
                "other": {
                    "anies": [
                        {
                            "value": "0.169005249960",
                            "module": "A1"
                        },
                        {
                            "value": "0.013011810356",
                            "module": "A2"
                        },
                        {
                            "value": "0.000623920280",
                            "module": "A3"
                        },
                        {
                            "value": "0.040371228090",
                            "module": "C1"
                        },
                        {
                            "value": "0.026498243540",
                            "module": "C2"
                        },
                        {
                            "value": "0.005355864134",
                            "module": "C3"
                        },
                        {
                            "value": "0.000543397956",
                            "module": "C4"
                        },
                        {
                            "value": "-0.016559763068",
                            "module": "D"
                        },
                        {
                            "name": "referenceToUnitGroupDataSet",
                            "value": {
                                "shortDescription": [
                                    {
                                        "value": "kg N eqv."
                                    }
                                ],
                                "type": "unit group data set",
                                "refObjectId": "d05bb823-ecdf-4686-8c40-bf1d9257859f",
                                "uri": "../unitgroups/d05bb823-ecdf-4686-8c40-bf1d9257859f"
                            }
                        }
                    ]
                }
            },
            {
                "referenceToLCIAMethodDataSet": {
                    "shortDescription": [
                        {
                            "value": "Eutrophication potential - freshwater (EP-freshwater)",
                            "lang": "en"
                        },
                        {
                            "value": "Overgj\u00f8dslingspotensial til ferskvann (EP-freshwater)",
                            "lang": "no"
                        }
                    ],
                    "type": "LCIA method data set",
                    "refObjectId": "b53ec18f-7377-4ad3-86eb-cc3f4f276b2b",
                    "version": "00.01.000"
                },
                "meanAmount": 0.0,
                "uncertaintyDistributionType": "undefined",
                "relativeStandardDeviation95In": 0,
                "other": {
                    "anies": [
                        {
                            "value": "0.007519161910",
                            "module": "A1"
                        },
                        {
                            "value": "0.000108265838",
                            "module": "A2"
                        },
                        {
                            "value": "0.000776442486",
                            "module": "A3"
                        },
                        {
                            "value": "0.000067697045",
                            "module": "C1"
                        },
                        {
                            "value": "0.000094780838",
                            "module": "C2"
                        },
                        {
                            "value": "0.000677693372",
                            "module": "C3"
                        },
                        {
                            "value": "0.000003840457",
                            "module": "C4"
                        },
                        {
                            "value": "-0.000841362359",
                            "module": "D"
                        },
                        {
                            "name": "referenceToUnitGroupDataSet",
                            "value": {
                                "shortDescription": [
                                    {
                                        "value": "kg P eqv."
                                    }
                                ],
                                "type": "unit group data set",
                                "refObjectId": "0429039d-a61d-4590-ba67-aa4a20a810a1",
                                "uri": "../unitgroups/0429039d-a61d-4590-ba67-aa4a20a810a1"
                            }
                        }
                    ]
                }
            },
            {
                "referenceToLCIAMethodDataSet": {
                    "shortDescription": [
                        {
                            "value": "Eutrophication potential - terrestrial (EP-terrestrial)",
                            "lang": "en"
                        },
                        {
                            "value": "Overgj\u00f8dslingspotensial til jord (EP-terrestrial)",
                            "lang": "no"
                        }
                    ],
                    "type": "LCIA method data set",
                    "refObjectId": "b5c614d2-def3-11e6-bf01-fe55135034f3",
                    "version": "00.01.000"
                },
                "meanAmount": 0.0,
                "uncertaintyDistributionType": "undefined",
                "relativeStandardDeviation95In": 0,
                "other": {
                    "anies": [
                        {
                            "value": "1.135332414893",
                            "module": "A1"
                        },
                        {
                            "value": "0.136028424719",
                            "module": "A2"
                        },
                        {
                            "value": "0.006783592517",
                            "module": "A3"
                        },
                        {
                            "value": "0.439042816317",
                            "module": "C1"
                        },
                        {
                            "value": "0.284707684849",
                            "module": "C2"
                        },
                        {
                            "value": "0.057574950983",
                            "module": "C3"
                        },
                        {
                            "value": "0.005903961936",
                            "module": "C4"
                        },
                        {
                            "value": "-0.179141490278",
                            "module": "D"
                        },
                        {
                            "name": "referenceToUnitGroupDataSet",
                            "value": {
                                "shortDescription": [
                                    {
                                        "value": "mol N eqv."
                                    }
                                ],
                                "type": "unit group data set",
                                "refObjectId": "71b4d617-0ec9-4d3f-b65e-e438940c2401",
                                "uri": "../unitgroups/71b4d617-0ec9-4d3f-b65e-e438940c2401"
                            }
                        }
                    ]
                }
            },
            {
                "referenceToLCIAMethodDataSet": {
                    "shortDescription": [
                        {
                            "value": "Potential Comparative Toxic Unit for humans - cancer effects (HTP-c)",
                            "lang": "en"
                        },
                        {
                            "value": "Toksisitet p\u00e5virkning p\u00e5 mennesker, kreft (HTP-c)",
                            "lang": "no"
                        }
                    ],
                    "type": "LCIA method data set",
                    "refObjectId": "2299222a-bbd8-474f-9d4f-4dd1f18aea7c",
                    "version": "00.01.000"
                },
                "meanAmount": 0.0,
                "uncertaintyDistributionType": "undefined",
                "relativeStandardDeviation95In": 0,
                "other": {
                    "anies": [
                        {
                            "value": "0.000000003050",
                            "module": "A1"
                        },
                        {
                            "value": "0.000000001093",
                            "module": "A2"
                        },
                        {
                            "value": "0.000000003729",
                            "module": "A3"
                        },
                        {
                            "value": "0.000000000504",
                            "module": "C1"
                        },
                        {
                            "value": "0.000000002504",
                            "module": "C2"
                        },
                        {
                            "value": "0.000000000377",
                            "module": "C3"
                        },
                        {
                            "value": "0.000000000010",
                            "module": "C4"
                        },
                        {
                            "value": "-0.000000001173",
                            "module": "D"
                        },
                        {
                            "name": "referenceToUnitGroupDataSet",
                            "value": {
                                "shortDescription": [
                                    {
                                        "value": "CTUh"
                                    }
                                ],
                                "type": "unit group data set",
                                "refObjectId": "d4c9523e-2d7e-49fd-8469-998f547d3a70",
                                "uri": "../unitgroups/d4c9523e-2d7e-49fd-8469-998f547d3a70"
                            }
                        }
                    ]
                }
            },
            {
                "referenceToLCIAMethodDataSet": {
                    "shortDescription": [
                        {
                            "value": "Potential Comparative Toxic Unit for humans - non-cancer effects (HTP-nc)",
                            "lang": "en"
                        },
                        {
                            "value": "Toksisitet p\u00e5virkning p\u00e5 mennesker, andre effekter enn kreft (HTP-nc) ",
                            "lang": "no"
                        }
                    ],
                    "type": "LCIA method data set",
                    "refObjectId": "3af763a5-b7a1-48c9-9cee-1f223481fcef",
                    "version": "00.01.000"
                },
                "meanAmount": 0.0,
                "uncertaintyDistributionType": "undefined",
                "relativeStandardDeviation95In": 0,
                "other": {
                    "anies": [
                        {
                            "value": "0.000000061380",
                            "module": "A1"
                        },
                        {
                            "value": "0.000000139405",
                            "module": "A2"
                        },
                        {
                            "value": "0.000000127070",
                            "module": "A3"
                        },
                        {
                            "value": "0.000000012587",
                            "module": "C1"
                        },
                        {
                            "value": "0.000000121820",
                            "module": "C2"
                        },
                        {
                            "value": "0.000000015665",
                            "module": "C3"
                        },
                        {
                            "value": "0.000000000232",
                            "module": "C4"
                        },
                        {
                            "value": "-0.000000021790",
                            "module": "D"
                        },
                        {
                            "name": "referenceToUnitGroupDataSet",
                            "value": {
                                "shortDescription": [
                                    {
                                        "value": "CTUh"
                                    }
                                ],
                                "type": "unit group data set",
                                "refObjectId": "d4c9523e-2d7e-49fd-8469-998f547d3a70",
                                "uri": "../unitgroups/d4c9523e-2d7e-49fd-8469-998f547d3a70"
                            }
                        }
                    ]
                }
            },
            {
                "referenceToLCIAMethodDataSet": {
                    "shortDescription": [
                        {
                            "value": "Potential Human exposure efficiency relative to U235 (IRP)",
                            "lang": "en"
                        },
                        {
                            "value": "Ioniserende str\u00e5ling, helseeffekt (IRP)",
                            "lang": "no"
                        }
                    ],
                    "type": "LCIA method data set",
                    "refObjectId": "b5c632be-def3-11e6-bf01-fe55135034f3",
                    "version": "00.01.000"
                },
                "meanAmount": 0.0,
                "uncertaintyDistributionType": "undefined",
                "relativeStandardDeviation95In": 0,
                "other": {
                    "anies": [
                        {
                            "value": "4.779535893413",
                            "module": "A1"
                        },
                        {
                            "value": "0.080094168051",
                            "module": "A2"
                        },
                        {
                            "value": "0.002038505809",
                            "module": "A3"
                        },
                        {
                            "value": "0.027435790960",
                            "module": "C1"
                        },
                        {
                            "value": "0.070118078120",
                            "module": "C2"
                        },
                        {
                            "value": "0.463670433681",
                            "module": "C3"
                        },
                        {
                            "value": "0.000454272267",
                            "module": "C4"
                        },
                        {
                            "value": "-0.369504948438",
                            "module": "D"
                        },
                        {
                            "name": "referenceToUnitGroupDataSet",
                            "value": {
                                "shortDescription": [
                                    {
                                        "value": "kBq U235 eqv."
                                    }
                                ],
                                "type": "unit group data set",
                                "refObjectId": "456b05bf-1415-44a9-9993-02452f554c09",
                                "uri": "../unitgroups/456b05bf-1415-44a9-9993-02452f554c09"
                            }
                        }
                    ]
                }
            },
            {
                "referenceToLCIAMethodDataSet": {
                    "shortDescription": [
                        {
                            "value": "Potential Soil quality index (SQP)",
                            "lang": "en"
                        },
                        {
                            "value": "P\u00e5virkninger knyttet til arealbruksendringer / jordkvalitet (SQP)",
                            "lang": "no"
                        }
                    ],
                    "type": "LCIA method data set",
                    "refObjectId": "b2ad6890-c78d-11e6-9d9d-cec0c932ce01",
                    "version": "00.01.000"
                },
                "meanAmount": 0.0,
                "uncertaintyDistributionType": "undefined",
                "relativeStandardDeviation95In": 0,
                "other": {
                    "anies": [
                        {
                            "value": "62.369866321455",
                            "module": "A1"
                        },
                        {
                            "value": "0.400923594507",
                            "module": "A2"
                        },
                        {
                            "value": "3.182680876918",
                            "module": "A3"
                        },
                        {
                            "value": "0.223423296106",
                            "module": "C1"
                        },
                        {
                            "value": "0.350986745314",
                            "module": "C2"
                        },
                        {
                            "value": "5.632861688265",
                            "module": "C3"
                        },
                        {
                            "value": "1.960812193814",
                            "module": "C4"
                        },
                        {
                            "value": "-65.321676055396",
                            "module": "D"
                        },
                        {
                            "name": "referenceToUnitGroupDataSet",
                            "value": {
                                "shortDescription": [
                                    {
                                        "value": "unitless"
                                    }
                                ],
                                "type": "unit group data set",
                                "refObjectId": "f130951c-e67f-4f7f-8dd4-665de3974e18",
                                "uri": "../unitgroups/f130951c-e67f-4f7f-8dd4-665de3974e18"
                            }
                        }
                    ]
                }
            },
            {
                "referenceToLCIAMethodDataSet": {
                    "shortDescription": [
                        {
                            "value": "Depletion potential of the stratospheric ozone layer (ODP)",
                            "lang": "en"
                        },
                        {
                            "value": "Potensial for nedbryting av stratosf\u00e6risk ozon (ODP)",
                            "lang": "no"
                        }
                    ],
                    "type": "LCIA method data set",
                    "refObjectId": "b5c629d6-def3-11e6-bf01-fe55135034f3",
                    "version": "00.01.000"
                },
                "meanAmount": 0.0,
                "uncertaintyDistributionType": "undefined",
                "relativeStandardDeviation95In": 0,
                "other": {
                    "anies": [
                        {
                            "value": "0.000009783966",
                            "module": "A1"
                        },
                        {
                            "value": "0.000000342816",
                            "module": "A2"
                        },
                        {
                            "value": "0.000000003137",
                            "module": "A3"
                        },
                        {
                            "value": "0.000000141536",
                            "module": "C1"
                        },
                        {
                            "value": "0.000000300116",
                            "module": "C2"
                        },
                        {
                            "value": "0.000000124614",
                            "module": "C3"
                        },
                        {
                            "value": "0.000000001911",
                            "module": "C4"
                        },
                        {
                            "value": "-0.000000138372",
                            "module": "D"
                        },
                        {
                            "name": "referenceToUnitGroupDataSet",
                            "value": {
                                "shortDescription": [
                                    {
                                        "value": "kg CFC 11 eqv."
                                    }
                                ],
                                "type": "unit group data set",
                                "refObjectId": "d9e957c9-7309-4474-bf3a-7777df6c4e5b",
                                "uri": "../unitgroups/d9e957c9-7309-4474-bf3a-7777df6c4e5b"
                            }
                        }
                    ]
                }
            },
            {
                "referenceToLCIAMethodDataSet": {
                    "shortDescription": [
                        {
                            "value": "Photochemical Ozone Creation Potential (POCP)",
                            "lang": "en"
                        },
                        {
                            "value": "Potensial for fotokjemisk oksidantdanning (POCP)",
                            "lang": "no"
                        }
                    ],
                    "type": "LCIA method data set",
                    "refObjectId": "b5c610fe-def3-11e6-bf01-fe55135034f3",
                    "version": "00.01.000"
                },
                "meanAmount": 0.0,
                "uncertaintyDistributionType": "undefined",
                "relativeStandardDeviation95In": 0,
                "other": {
                    "anies": [
                        {
                            "value": "0.476017386893",
                            "module": "A1"
                        },
                        {
                            "value": "0.058233682977",
                            "module": "A2"
                        },
                        {
                            "value": "0.002055772743",
                            "module": "A3"
                        },
                        {
                            "value": "0.129186980212",
                            "module": "C1"
                        },
                        {
                            "value": "0.091350516755",
                            "module": "C2"
                        },
                        {
                            "value": "0.021576542053",
                            "module": "C3"
                        },
                        {
                            "value": "0.001767213886",
                            "module": "C4"
                        },
                        {
                            "value": "-0.058514845593",
                            "module": "D"
                        },
                        {
                            "name": "referenceToUnitGroupDataSet",
                            "value": {
                                "shortDescription": [
                                    {
                                        "value": "kg NMVOC eqv."
                                    }
                                ],
                                "type": "unit group data set",
                                "refObjectId": "d27c25f8-fbc1-44c6-b47b-4adbae4199c6",
                                "uri": "../unitgroups/d27c25f8-fbc1-44c6-b47b-4adbae4199c6"
                            }
                        }
                    ]
                }
            },
            {
                "referenceToLCIAMethodDataSet": {
                    "shortDescription": [
                        {
                            "value": "Abiotic depletion potential - fossil resources (ADPF)",
                            "lang": "en"
                        },
                        {
                            "value": "Abiotisk utarmingspotensial for fossile ressurser, fosile brensler (ADP-fossil)",
                            "lang": "no"
                        }
                    ],
                    "type": "LCIA method data set",
                    "refObjectId": "b2ad6110-c78d-11e6-9d9d-cec0c932ce01",
                    "version": "00.01.000"
                },
                "meanAmount": 0.0,
                "uncertaintyDistributionType": "undefined",
                "relativeStandardDeviation95In": 0,
                "other": {
                    "anies": [
                        {
                            "value": "864.152922208510",
                            "module": "A1"
                        },
                        {
                            "value": "210.968028876740",
                            "module": "A2"
                        },
                        {
                            "value": "2.143974075364",
                            "module": "A3"
                        },
                        {
                            "value": "118.141939161400",
                            "module": "C1"
                        },
                        {
                            "value": "184.691016809055",
                            "module": "C2"
                        },
                        {
                            "value": "82.375307199885",
                            "module": "C3"
                        },
                        {
                            "value": "1.650960983953",
                            "module": "C4"
                        },
                        {
                            "value": "-104.634054675997",
                            "module": "D"
                        },
                        {
                            "name": "referenceToUnitGroupDataSet",
                            "value": {
                                "shortDescription": [
                                    {
                                        "value": "MJ"
                                    }
                                ],
                                "type": "unit group data set",
                                "refObjectId": "93a60a57-a3c8-11da-a746-0800200c9a66",
                                "uri": "../unitgroups/93a60a57-a3c8-11da-a746-0800200c9a66"
                            }
                        }
                    ]
                }
            },
            {
                "referenceToLCIAMethodDataSet": {
                    "shortDescription": [
                        {
                            "value": "Abiotic depletion potential - non-fossil resources (ADPE)",
                            "lang": "en"
                        },
                        {
                            "value": "Abiotisk utarmingspotensial for ikke-fossile ressurser, mineraler (ADP-elements)",
                            "lang": "no"
                        }
                    ],
                    "type": "LCIA method data set",
                    "refObjectId": "b2ad6494-c78d-11e6-9d9d-cec0c932ce01",
                    "version": "00.01.000"
                },
                "meanAmount": 0.0,
                "uncertaintyDistributionType": "undefined",
                "relativeStandardDeviation95In": 0,
                "other": {
                    "anies": [
                        {
                            "value": "0.000129922448",
                            "module": "A1"
                        },
                        {
                            "value": "0.000000545410",
                            "module": "A2"
                        },
                        {
                            "value": "0.000000005694",
                            "module": "A3"
                        },
                        {
                            "value": "0.000000377181",
                            "module": "C1"
                        },
                        {
                            "value": "0.000000477477",
                            "module": "C2"
                        },
                        {
                            "value": "0.000000083638",
                            "module": "C3"
                        },
                        {
                            "value": "0.000000005105",
                            "module": "C4"
                        },
                        {
                            "value": "-0.000000631201",
                            "module": "D"
                        },
                        {
                            "name": "referenceToUnitGroupDataSet",
                            "value": {
                                "shortDescription": [
                                    {
                                        "value": "kg Sb-eqv."
                                    }
                                ],
                                "type": "unit group data set",
                                "refObjectId": "54ccd2d9-a32a-4fc2-923d-f2c8c93e89d4",
                                "uri": "../unitgroups/54ccd2d9-a32a-4fc2-923d-f2c8c93e89d4"
                            }
                        }
                    ]
                }
            },
            {
                "referenceToLCIAMethodDataSet": {
                    "shortDescription": [
                        {
                            "value": "Water (user) deprivation potential (WDP)",
                            "lang": "en"
                        },
                        {
                            "value": "Utarmingspotensial for vannressurser (WDP)",
                            "lang": "no"
                        }
                    ],
                    "type": "LCIA method data set",
                    "refObjectId": "b2ad66ce-c78d-11e6-9d9d-cec0c932ce01",
                    "version": "00.01.000"
                },
                "meanAmount": 0.0,
                "uncertaintyDistributionType": "undefined",
                "relativeStandardDeviation95In": 0,
                "other": {
                    "anies": [
                        {
                            "value": "140.537371490538",
                            "module": "A1"
                        },
                        {
                            "value": "0.193156307521",
                            "module": "A2"
                        },
                        {
                            "value": "14.936297614981",
                            "module": "A3"
                        },
                        {
                            "value": "0.151317677959",
                            "module": "C1"
                        },
                        {
                            "value": "0.169097818096",
                            "module": "C2"
                        },
                        {
                            "value": "1.319742150457",
                            "module": "C3"
                        },
                        {
                            "value": "0.002275996095",
                            "module": "C4"
                        },
                        {
                            "value": "-143.872892942509",
                            "module": "D"
                        },
                        {
                            "name": "referenceToUnitGroupDataSet",
                            "value": {
                                "shortDescription": [
                                    {
                                        "value": "m3 world eqv."
                                    }
                                ],
                                "type": "unit group data set",
                                "refObjectId": "6ae2df01-888e-46c8-b17d-49fa3869b476",
                                "uri": "../unitgroups/6ae2df01-888e-46c8-b17d-49fa3869b476"
                            }
                        }
                    ]
                }
            },
            {
                "referenceToLCIAMethodDataSet": {
                    "shortDescription": [
                        {
                            "value": "Global warming potential except emissions and uptake of biogenic carbon (GWP-IOBC/GHG)",
                            "lang": "en"
                        },
                        {
                            "value": "Globalt oppvarmingspotensial beregnet etter prinsippet om umiddelbar oksidasjon (GWP-IOBC)",
                            "lang": "no"
                        }
                    ],
                    "type": "LCIA method data set",
                    "refObjectId": "fb774615-0575-45de-9a89-1ded92f19770",
                    "version": "00.01.000"
                },
                "meanAmount": 0.0,
                "uncertaintyDistributionType": "undefined",
                "relativeStandardDeviation95In": 0,
                "other": {
                    "anies": [
                        {
                            "name": "referenceToUnitGroupDataSet",
                            "value": {
                                "shortDescription": [
                                    {
                                        "value": "kg CO2 eqv."
                                    }
                                ],
                                "type": "unit group data set",
                                "refObjectId": "1ebf3012-d0db-4de2-aefd-ef30cedb0be1",
                                "uri": "../unitgroups/1ebf3012-d0db-4de2-aefd-ef30cedb0be1"
                            }
                        }
                    ]
                }
            }
        ]
    },
    "otherAttributes": {
        "{http://www.indata.network/EPD/2019}epd-version": "1.2"
    },
    "version": "1.1"
}