{
    "processInformation": {
        "dataSetInformation": {
            "UUID": "7f73caec-8a20-41d2-9b7d-16c368bfe27e",
            "name": {
                "baseName": [
                    {
                        "value": " Birsta S N2 W4 c/c4  m",
                        "lang": "en"
                    }
                ]
            },
            "classificationInformation": {
                "classification": [
                    {
                        "class": [
                            {
                                "value": "Bygg",
                                "level": 0,
                                "classId": "f0167df9-d436-462f-9969-0234c152f514"
                            },
                            {
                                "value": "St\u00e5l-, aluminiumskonstruksjoner",
                                "level": 1,
                                "classId": "992467c5-eec4-4d69-88ba-672f1a896481"
                            }
                        ],
                        "name": "EPDNorge"
                    }
                ]
            },
            "generalComment": [
                {
                    "value": "Data quality:\nSpecific data for the product composition are provided by the manufacturer. The data represent the production of the declared product and were collected for EPD development in the year of study. Background data is based on EPDs according to EN 15804 and different LCA databases. The data quality of the raw materials in A1 is presented in the table below.\n\nAllocation:\nThe allocation is made in accordance with the provisions of EN 15804. Incoming energy and water and waste production in-house is allocated equally among all products through mass allocation. Effects of primary production of recycled materials is allocated to the main product in which the material was used. The recycling process and transportation of the material is allocated to this analysis.\n\nCut-off criteria:\nAll major raw materials and all the essential energy is included. The production processes for raw materials and energy flows with very small amounts (less than 1%) are not included. These cut-off criteria do not\napply for hazardous materials and substances.\n",
                    "lang": "en"
                }
            ]
        },
        "quantitativeReference": {
            "referenceToReferenceFlow": [
                1
            ],
            "type": "Reference flow(s)"
        },
        "time": {
            "referenceYear": 2024,
            "dataSetValidUntil": 2029,
            "timeRepresentativenessDescription": [
                {
                    "value": "\"2024-06-24\" - \"2029-06-24\"",
                    "lang": "en"
                }
            ],
            "other": {
                "anies": [
                    {
                        "name": "publicationDateOfEPD",
                        "value": 1719187200000
                    }
                ]
            }
        },
        "geography": {
            "locationOfOperationSupplyOrProduction": {
                "descriptionOfRestrictions": [
                    {
                        "value": "Sweden",
                        "lang": "en"
                    }
                ],
                "location": "CN"
            }
        },
        "technology": {
            "technologicalApplicability": [
                {
                    "value": "Birsta S - where S stands for \"snow resistant\" - is a railing that\nis specially manufactured to cope with close contact with snow ploughs.\nIt can also be advantageously used as collision protection\nat e.g. car parks, industrial areas and warehouse buildings.",
                    "lang": "en"
                }
            ]
        }
    },
    "modellingAndValidation": {
        "LCIMethodAndAllocation": {
            "typeOfDataSet": "EPD",
            "referenceToLCAMethodDetails": [
                {
                    "shortDescription": [
                        {
                            "value": "NPCR 013:2021 Part B for Steel and aluminium construction products",
                            "lang": "en"
                        }
                    ],
                    "type": "source data set",
                    "refObjectId": "da909e71-8481-4aaa-8729-c8dd9e3bd9ff",
                    "version": "00.00.000"
                }
            ],
            "other": {
                "anies": [
                    {
                        "name": "subType",
                        "value": "specific dataset"
                    }
                ]
            }
        },
        "dataSourcesTreatmentAndRepresentativeness": {
            "referenceToDataSource": [
                {
                    "shortDescription": [
                        {
                            "value": "NEPD-4311-3545_BFOU-M-06-1kV-3X-4-6mm-.pdf",
                            "lang": "en"
                        }
                    ],
                    "type": "source data set",
                    "refObjectId": "b497a91f-e14b-4b69-8f28-f50eb1576766",
                    "version": "00.96.001",
                    "uri": "http://openlca.org/ilcd/resource/sources/b497a91f-e14b-4b69-8f28-f50eb1576766"
                }
            ],
            "useAdviceForDataSet": [
                {
                    "value": "A1-A5 C1-C5 D",
                    "lang": "en"
                }
            ],
            "other": {
                "anies": [
                    {
                        "name": "referenceToOriginalEPD",
                        "value": {
                            "shortDescription": [
                                {
                                    "value": "NEPD-6940-6338",
                                    "lang": "en"
                                }
                            ],
                            "type": "source data set",
                            "refObjectId": "0548184e-58ba-4d56-ab4e-41599b772f61",
                            "version": "00.00.000"
                        }
                    }
                ]
            }
        },
        "validation": {
            "review": [
                {
                    "referenceToNameOfReviewerAndInstitution": [
                        {
                            "shortDescription": [
                                {
                                    "value": "Alexander Borg",
                                    "lang": "en"
                                }
                            ],
                            "type": "contact data set",
                            "refObjectId": "885690c3-edf3-408c-9a55-cae86e1f4180",
                            "version": "00.00.001"
                        }
                    ],
                    "type": "Independent external review"
                }
            ]
        },
        "complianceDeclarations": {
            "compliance": [
                {
                    "referenceToComplianceSystem": {
                        "shortDescription": [
                            {
                                "value": "EN 15804+A2",
                                "lang": "en"
                            }
                        ],
                        "type": "source data set",
                        "refObjectId": "c0016b33-8cf7-415c-ac6e-deba0d21440d",
                        "version": "00.02.000"
                    },
                    "approvalOfOverallCompliance": "Fully compliant",
                    "nomenclatureCompliance": "Fully compliant",
                    "methodologicalCompliance": "Fully compliant",
                    "reviewCompliance": "Fully compliant",
                    "documentationCompliance": "Fully compliant",
                    "qualityCompliance": "Fully compliant"
                },
                {
                    "referenceToComplianceSystem": {
                        "shortDescription": [
                            {
                                "value": "ISO 14025",
                                "lang": "en"
                            }
                        ],
                        "type": "source data set",
                        "refObjectId": "4f2eb655-6e44-4874-a95a-e28f5442cd4d",
                        "version": "00.00.001"
                    },
                    "approvalOfOverallCompliance": "Fully compliant",
                    "nomenclatureCompliance": "Fully compliant",
                    "methodologicalCompliance": "Fully compliant",
                    "reviewCompliance": "Fully compliant",
                    "documentationCompliance": "Fully compliant",
                    "qualityCompliance": "Fully compliant"
                },
                {
                    "referenceToComplianceSystem": {
                        "shortDescription": [
                            {
                                "value": "ISO 21930",
                                "lang": "en"
                            }
                        ],
                        "type": "source data set",
                        "refObjectId": "9c1e8451-2321-4498-b459-b6568b6b6547",
                        "version": "00.00.001"
                    },
                    "approvalOfOverallCompliance": "Fully compliant",
                    "nomenclatureCompliance": "Fully compliant",
                    "methodologicalCompliance": "Fully compliant",
                    "reviewCompliance": "Fully compliant",
                    "documentationCompliance": "Fully compliant",
                    "qualityCompliance": "Fully compliant"
                }
            ]
        }
    },
    "administrativeInformation": {
        "dataGenerator": {
            "referenceToPersonOrEntityGeneratingTheDataSet": [
                {
                    "shortDescription": [
                        {
                            "value": "LCA.no AS",
                            "lang": "en"
                        }
                    ],
                    "type": "contact data set",
                    "refObjectId": "77a6868e-b256-47c8-a410-32706b6e1814",
                    "version": "00.00.001"
                }
            ]
        },
        "dataEntryBy": {
            "timeStamp": 1724001632000,
            "referenceToDataSetFormat": [
                {
                    "shortDescription": [
                        {
                            "value": "ILCD format",
                            "lang": "en"
                        }
                    ],
                    "type": "source data set",
                    "refObjectId": "a97a0155-0234-4b87-b4ce-a45da52f2a40",
                    "version": "01.00.000",
                    "uri": "http://lca.jrc.ec.europa.eu/lcainfohub/sample_data/ilcd/sources/ILCD_Format_a97a0155-0234-4b87-b4ce-a45da52f2a40_01.00.000.xml"
                },
                {
                    "shortDescription": [
                        {
                            "value": "EPD Data Format Extensions v1.2",
                            "lang": "no"
                        },
                        {
                            "value": "EPD Data Format Extensions v1.2",
                            "lang": "en"
                        },
                        {
                            "value": "EPD-Datenformaterweiterungen v1.2",
                            "lang": "de"
                        }
                    ],
                    "type": "source data set",
                    "refObjectId": "a29449fd-aa2f-4de8-b5d7-4b06b43c6fde",
                    "version": "00.01.000"
                }
            ]
        },
        "publicationAndOwnership": {
            "dataSetVersion": "00.03.000",
            "dateOfLastRevision": 1718806142802,
            "referenceToRegistrationAuthority": {
                "shortDescription": [
                    {
                        "value": "EPD Norway",
                        "lang": "en"
                    }
                ],
                "type": "contact data set",
                "refObjectId": "7008caa3-6fea-4ad2-81eb-f2b7a0610e6c",
                "version": "00.00.004"
            },
            "registrationNumber": "NEPD-6940-6338",
            "referenceToOwnershipOfDataSet": {
                "shortDescription": [
                    {
                        "value": "Saferoad Sverige AB",
                        "lang": "en"
                    }
                ],
                "type": "contact data set",
                "refObjectId": "89cd70c2-e3df-4ea2-a2d9-3cf671b6d59f",
                "version": "00.00.000"
            },
            "copyright": true,
            "licenseType": "Free of charge for all users and uses",
            "accessRestrictions": [
                {
                    "value": "None",
                    "lang": "en"
                }
            ],
            "other": {
                "anies": [
                    {
                        "name": "referenceToPublisher",
                        "value": {
                            "shortDescription": [
                                {
                                    "value": "EPD Norway",
                                    "lang": "en"
                                }
                            ],
                            "type": "contact data set",
                            "refObjectId": "7008caa3-6fea-4ad2-81eb-f2b7a0610e6c",
                            "version": "00.00.004"
                        }
                    }
                ]
            }
        }
    },
    "exchanges": {
        "exchange": [
            {
                "referenceToFlowDataSet": {
                    "shortDescription": [
                        {
                            "value": " Birsta S N2 W4 c/c4  m",
                            "lang": "en"
                        }
                    ],
                    "type": "flow data set",
                    "refObjectId": "09979d9b-3f59-493e-a856-258ed21fe665",
                    "version": "00.01.000"
                },
                "functionType": "General reminder flow",
                "exchangeDirection": "Output",
                "meanAmount": 1.0,
                "resultingAmount": 1.0,
                "minimumAmount": 0.0,
                "maximumAmount": 0.0,
                "uncertaintyDistributionType": "undefined",
                "relativeStandardDeviation95In": 0,
                "dataSourceType": "Primary",
                "dataDerivationTypeStatus": "Measured",
                "dataSetInternalID": 1
            },
            {
                "referenceToFlowDataSet": {
                    "shortDescription": [
                        {
                            "value": "Use of renewable primary energy (PERE)",
                            "lang": "en"
                        },
                        {
                            "value": "Fornybar prim\u00e6renergi brukt som energib\u00e6rer (RPEE)",
                            "lang": "no"
                        }
                    ],
                    "type": "flow data set",
                    "refObjectId": "20f32be5-0398-4288-9b6d-accddd195317",
                    "version": "30.00.000"
                },
                "functionType": "General reminder flow",
                "exchangeDirection": "Input",
                "meanAmount": 0.0,
                "resultingAmount": 0.0,
                "minimumAmount": 0.0,
                "maximumAmount": 0.0,
                "uncertaintyDistributionType": "undefined",
                "relativeStandardDeviation95In": 0,
                "dataSourceType": "Primary",
                "dataDerivationTypeStatus": "Measured",
                "other": {
                    "anies": [
                        {
                            "value": "27.910681274414",
                            "module": "A1-A3"
                        },
                        {
                            "value": "0.049830172000",
                            "module": "A4"
                        },
                        {
                            "value": "0.073676717519",
                            "module": "A5"
                        },
                        {
                            "value": "0.073676717519",
                            "module": "C1"
                        },
                        {
                            "value": "0.049830172000",
                            "module": "C2"
                        },
                        {
                            "value": "0.000000000000",
                            "module": "C3"
                        },
                        {
                            "value": "0.002977063365",
                            "module": "C4"
                        },
                        {
                            "value": "-5.801211270039",
                            "module": "D"
                        },
                        {
                            "name": "referenceToUnitGroupDataSet",
                            "value": {
                                "shortDescription": [
                                    {
                                        "value": "MJ"
                                    }
                                ],
                                "type": "unit group data set",
                                "refObjectId": "93a60a57-a3c8-11da-a746-0800200c9a66",
                                "uri": "../unitgroups/93a60a57-a3c8-11da-a746-0800200c9a66"
                            }
                        }
                    ]
                },
                "dataSetInternalID": 2
            },
            {
                "referenceToFlowDataSet": {
                    "shortDescription": [
                        {
                            "value": "Use of renewable primary energy resources used as raw materials (PERM)",
                            "lang": "en"
                        },
                        {
                            "value": "Fornybar prim\u00e6renergi brukt som energib\u00e6rer (RPEE)",
                            "lang": "no"
                        }
                    ],
                    "type": "flow data set",
                    "refObjectId": "fb3ec0de-548d-4508-aea5-00b73bf6f702",
                    "version": "30.00.000"
                },
                "functionType": "General reminder flow",
                "exchangeDirection": "Input",
                "meanAmount": 0.0,
                "resultingAmount": 0.0,
                "minimumAmount": 0.0,
                "maximumAmount": 0.0,
                "uncertaintyDistributionType": "undefined",
                "relativeStandardDeviation95In": 0,
                "dataSourceType": "Primary",
                "dataDerivationTypeStatus": "Measured",
                "other": {
                    "anies": [
                        {
                            "value": "0.000000000000",
                            "module": "A1-A3"
                        },
                        {
                            "value": "0.000000000000",
                            "module": "A4"
                        },
                        {
                            "value": "0.000000000000",
                            "module": "A5"
                        },
                        {
                            "value": "0.000000000000",
                            "module": "C1"
                        },
                        {
                            "value": "0.000000000000",
                            "module": "C2"
                        },
                        {
                            "value": "0.000000000000",
                            "module": "C3"
                        },
                        {
                            "value": "0.000000000000",
                            "module": "C4"
                        },
                        {
                            "value": "0.000000000000",
                            "module": "D"
                        },
                        {
                            "name": "referenceToUnitGroupDataSet",
                            "value": {
                                "shortDescription": [
                                    {
                                        "value": "MJ"
                                    }
                                ],
                                "type": "unit group data set",
                                "refObjectId": "93a60a57-a3c8-11da-a746-0800200c9a66",
                                "uri": "../unitgroups/93a60a57-a3c8-11da-a746-0800200c9a66"
                            }
                        }
                    ]
                },
                "dataSetInternalID": 3
            },
            {
                "referenceToFlowDataSet": {
                    "shortDescription": [
                        {
                            "value": "Total use of renewable primary energy resource (PERT)",
                            "lang": "en"
                        },
                        {
                            "value": "Total bruk av fornybar prim\u00e6renergi (TPE)",
                            "lang": "no"
                        }
                    ],
                    "type": "flow data set",
                    "refObjectId": "53f97275-fa8a-4cdd-9024-65936002acd0",
                    "version": "30.00.000"
                },
                "functionType": "General reminder flow",
                "exchangeDirection": "Input",
                "meanAmount": 0.0,
                "resultingAmount": 0.0,
                "minimumAmount": 0.0,
                "maximumAmount": 0.0,
                "uncertaintyDistributionType": "undefined",
                "relativeStandardDeviation95In": 0,
                "dataSourceType": "Primary",
                "dataDerivationTypeStatus": "Measured",
                "other": {
                    "anies": [
                        {
                            "value": "27.910681274414",
                            "module": "A1-A3"
                        },
                        {
                            "value": "0.049830172000",
                            "module": "A4"
                        },
                        {
                            "value": "0.073676717519",
                            "module": "A5"
                        },
                        {
                            "value": "0.073676717519",
                            "module": "C1"
                        },
                        {
                            "value": "0.049830172000",
                            "module": "C2"
                        },
                        {
                            "value": "0.000000000000",
                            "module": "C3"
                        },
                        {
                            "value": "0.002977063365",
                            "module": "C4"
                        },
                        {
                            "value": "-5.801211270039",
                            "module": "D"
                        },
                        {
                            "name": "referenceToUnitGroupDataSet",
                            "value": {
                                "shortDescription": [
                                    {
                                        "value": "MJ"
                                    }
                                ],
                                "type": "unit group data set",
                                "refObjectId": "93a60a57-a3c8-11da-a746-0800200c9a66",
                                "uri": "../unitgroups/93a60a57-a3c8-11da-a746-0800200c9a66"
                            }
                        }
                    ]
                },
                "dataSetInternalID": 4
            },
            {
                "referenceToFlowDataSet": {
                    "shortDescription": [
                        {
                            "value": "Use of non renewable primary energy (PENRE)",
                            "lang": "en"
                        },
                        {
                            "value": "Ikke fornybar prim\u00e6renergi brukt som energib\u00e6rer (NRPE)",
                            "lang": "no"
                        }
                    ],
                    "type": "flow data set",
                    "refObjectId": "ac857178-2b45-46ec-892a-a9a4332f0372",
                    "version": "30.00.000"
                },
                "functionType": "General reminder flow",
                "exchangeDirection": "Input",
                "meanAmount": 0.0,
                "resultingAmount": 0.0,
                "minimumAmount": 0.0,
                "maximumAmount": 0.0,
                "uncertaintyDistributionType": "undefined",
                "relativeStandardDeviation95In": 0,
                "dataSourceType": "Primary",
                "dataDerivationTypeStatus": "Measured",
                "other": {
                    "anies": [
                        {
                            "value": "343.072753803821",
                            "module": "A1-A3"
                        },
                        {
                            "value": "3.961583544800",
                            "module": "A4"
                        },
                        {
                            "value": "13.621171823158",
                            "module": "A5"
                        },
                        {
                            "value": "13.621171823158",
                            "module": "C1"
                        },
                        {
                            "value": "3.961583544800",
                            "module": "C2"
                        },
                        {
                            "value": "0.000000000000",
                            "module": "C3"
                        },
                        {
                            "value": "0.193447348859",
                            "module": "C4"
                        },
                        {
                            "value": "-50.963167943253",
                            "module": "D"
                        },
                        {
                            "name": "referenceToUnitGroupDataSet",
                            "value": {
                                "shortDescription": [
                                    {
                                        "value": "MJ"
                                    }
                                ],
                                "type": "unit group data set",
                                "refObjectId": "93a60a57-a3c8-11da-a746-0800200c9a66",
                                "uri": "../unitgroups/93a60a57-a3c8-11da-a746-0800200c9a66"
                            }
                        }
                    ]
                },
                "dataSetInternalID": 5
            },
            {
                "referenceToFlowDataSet": {
                    "shortDescription": [
                        {
                            "value": "Use of non renewable primary energy resources used as raw materials (PENRM)",
                            "lang": "en"
                        },
                        {
                            "value": "Ikke fornybar prim\u00e6renergi brukt som r\u00e5materiale (NRPM)",
                            "lang": "no"
                        }
                    ],
                    "type": "flow data set",
                    "refObjectId": "1421caa0-679d-4bf4-b282-0eb850ccae27",
                    "version": "30.00.000"
                },
                "functionType": "General reminder flow",
                "exchangeDirection": "Input",
                "meanAmount": 0.0,
                "resultingAmount": 0.0,
                "minimumAmount": 0.0,
                "maximumAmount": 0.0,
                "uncertaintyDistributionType": "undefined",
                "relativeStandardDeviation95In": 0,
                "dataSourceType": "Primary",
                "dataDerivationTypeStatus": "Measured",
                "other": {
                    "anies": [
                        {
                            "value": "0.000000000000",
                            "module": "A1-A3"
                        },
                        {
                            "value": "0.000000000000",
                            "module": "A4"
                        },
                        {
                            "value": "0.000000000000",
                            "module": "A5"
                        },
                        {
                            "value": "0.000000000000",
                            "module": "C1"
                        },
                        {
                            "value": "0.000000000000",
                            "module": "C2"
                        },
                        {
                            "value": "0.000000000000",
                            "module": "C3"
                        },
                        {
                            "value": "0.000000000000",
                            "module": "C4"
                        },
                        {
                            "value": "0.000000000000",
                            "module": "D"
                        },
                        {
                            "name": "referenceToUnitGroupDataSet",
                            "value": {
                                "shortDescription": [
                                    {
                                        "value": "MJ"
                                    }
                                ],
                                "type": "unit group data set",
                                "refObjectId": "93a60a57-a3c8-11da-a746-0800200c9a66",
                                "uri": "../unitgroups/93a60a57-a3c8-11da-a746-0800200c9a66"
                            }
                        }
                    ]
                },
                "dataSetInternalID": 6
            },
            {
                "referenceToFlowDataSet": {
                    "shortDescription": [
                        {
                            "value": "Total use of non renewable primary energy resource (PENRT)",
                            "lang": "en"
                        },
                        {
                            "value": "Total nicht erneuerbare Prim\u00e4renergie (PENRT)",
                            "lang": "no"
                        }
                    ],
                    "type": "flow data set",
                    "refObjectId": "06159210-646b-4c8d-8583-da9b3b95a6c1",
                    "version": "30.00.000"
                },
                "functionType": "General reminder flow",
                "exchangeDirection": "Input",
                "meanAmount": 0.0,
                "resultingAmount": 0.0,
                "minimumAmount": 0.0,
                "maximumAmount": 0.0,
                "uncertaintyDistributionType": "undefined",
                "relativeStandardDeviation95In": 0,
                "dataSourceType": "Primary",
                "dataDerivationTypeStatus": "Measured",
                "other": {
                    "anies": [
                        {
                            "value": "343.072753803821",
                            "module": "A1-A3"
                        },
                        {
                            "value": "3.961583544800",
                            "module": "A4"
                        },
                        {
                            "value": "13.621171823158",
                            "module": "A5"
                        },
                        {
                            "value": "13.621171823158",
                            "module": "C1"
                        },
                        {
                            "value": "3.961583544800",
                            "module": "C2"
                        },
                        {
                            "value": "0.000000000000",
                            "module": "C3"
                        },
                        {
                            "value": "0.193447348859",
                            "module": "C4"
                        },
                        {
                            "value": "-50.963167943253",
                            "module": "D"
                        },
                        {
                            "name": "referenceToUnitGroupDataSet",
                            "value": {
                                "shortDescription": [
                                    {
                                        "value": "MJ"
                                    }
                                ],
                                "type": "unit group data set",
                                "refObjectId": "93a60a57-a3c8-11da-a746-0800200c9a66",
                                "uri": "../unitgroups/93a60a57-a3c8-11da-a746-0800200c9a66"
                            }
                        }
                    ]
                },
                "dataSetInternalID": 7
            },
            {
                "referenceToFlowDataSet": {
                    "shortDescription": [
                        {
                            "value": "Use of secondary material (SM)",
                            "lang": "en"
                        },
                        {
                            "value": "Bruk av sekund\u00e6re materialer (SM)",
                            "lang": "no"
                        }
                    ],
                    "type": "flow data set",
                    "refObjectId": "c6a1f35f-2d09-4f54-8dfb-97e502e1ce92",
                    "version": "30.00.000"
                },
                "functionType": "General reminder flow",
                "exchangeDirection": "Input",
                "meanAmount": 0.0,
                "resultingAmount": 0.0,
                "minimumAmount": 0.0,
                "maximumAmount": 0.0,
                "uncertaintyDistributionType": "undefined",
                "relativeStandardDeviation95In": 0,
                "dataSourceType": "Primary",
                "dataDerivationTypeStatus": "Measured",
                "other": {
                    "anies": [
                        {
                            "value": "10.225510565629",
                            "module": "A1-A3"
                        },
                        {
                            "value": "0.000000000000",
                            "module": "A4"
                        },
                        {
                            "value": "0.000000000000",
                            "module": "A5"
                        },
                        {
                            "value": "0.000000000000",
                            "module": "C1"
                        },
                        {
                            "value": "0.000000000000",
                            "module": "C2"
                        },
                        {
                            "value": "0.000000000000",
                            "module": "C3"
                        },
                        {
                            "value": "0.000000000000",
                            "module": "C4"
                        },
                        {
                            "value": "0.000000000000",
                            "module": "D"
                        },
                        {
                            "name": "referenceToUnitGroupDataSet",
                            "value": {
                                "shortDescription": [
                                    {
                                        "value": "kg"
                                    }
                                ],
                                "type": "unit group data set",
                                "refObjectId": "ad38d542-3fe9-439d-9b95-2f5f7752acaf",
                                "uri": "../unitgroups/ad38d542-3fe9-439d-9b95-2f5f7752acaf"
                            }
                        }
                    ]
                },
                "dataSetInternalID": 8
            },
            {
                "referenceToFlowDataSet": {
                    "shortDescription": [
                        {
                            "value": "Use of renewable secondary fuels (RSF)",
                            "lang": "en"
                        },
                        {
                            "value": "Bruk av fornybart sekund\u00e6re brensel (RSF)",
                            "lang": "no"
                        }
                    ],
                    "type": "flow data set",
                    "refObjectId": "64333088-a55f-4aa2-9a31-c10b07816787",
                    "version": "30.00.000"
                },
                "functionType": "General reminder flow",
                "exchangeDirection": "Input",
                "meanAmount": 0.0,
                "resultingAmount": 0.0,
                "minimumAmount": 0.0,
                "maximumAmount": 0.0,
                "uncertaintyDistributionType": "undefined",
                "relativeStandardDeviation95In": 0,
                "dataSourceType": "Primary",
                "dataDerivationTypeStatus": "Measured",
                "other": {
                    "anies": [
                        {
                            "value": "0.359932595248",
                            "module": "A1-A3"
                        },
                        {
                            "value": "0.001743016800",
                            "module": "A4"
                        },
                        {
                            "value": "0.001812504474",
                            "module": "A5"
                        },
                        {
                            "value": "0.001812504474",
                            "module": "C1"
                        },
                        {
                            "value": "0.001743016800",
                            "module": "C2"
                        },
                        {
                            "value": "0.000000000000",
                            "module": "C3"
                        },
                        {
                            "value": "0.000061512185",
                            "module": "C4"
                        },
                        {
                            "value": "-0.034429204998",
                            "module": "D"
                        },
                        {
                            "name": "referenceToUnitGroupDataSet",
                            "value": {
                                "shortDescription": [
                                    {
                                        "value": "MJ"
                                    }
                                ],
                                "type": "unit group data set",
                                "refObjectId": "93a60a57-a3c8-11da-a746-0800200c9a66",
                                "uri": "../unitgroups/93a60a57-a3c8-11da-a746-0800200c9a66"
                            }
                        }
                    ]
                },
                "dataSetInternalID": 9
            },
            {
                "referenceToFlowDataSet": {
                    "shortDescription": [
                        {
                            "value": "Use of non renewable secondary fuels (NRSF)",
                            "lang": "en"
                        },
                        {
                            "value": "Bruk av ikke fornybart sekund\u00e6re brensel (NRSF)",
                            "lang": "no"
                        }
                    ],
                    "type": "flow data set",
                    "refObjectId": "89def144-d39a-4287-b86f-efde453ddcb2",
                    "version": "30.00.000"
                },
                "functionType": "General reminder flow",
                "exchangeDirection": "Input",
                "meanAmount": 0.0,
                "resultingAmount": 0.0,
                "minimumAmount": 0.0,
                "maximumAmount": 0.0,
                "uncertaintyDistributionType": "undefined",
                "relativeStandardDeviation95In": 0,
                "dataSourceType": "Primary",
                "dataDerivationTypeStatus": "Measured",
                "other": {
                    "anies": [
                        {
                            "value": "10.253284572571",
                            "module": "A1-A3"
                        },
                        {
                            "value": "0.005841864000",
                            "module": "A4"
                        },
                        {
                            "value": "0.026671257942",
                            "module": "A5"
                        },
                        {
                            "value": "0.026671257942",
                            "module": "C1"
                        },
                        {
                            "value": "0.005841864000",
                            "module": "C2"
                        },
                        {
                            "value": "0.000000000000",
                            "module": "C3"
                        },
                        {
                            "value": "0.000176880865",
                            "module": "C4"
                        },
                        {
                            "value": "2.269028111378",
                            "module": "D"
                        },
                        {
                            "name": "referenceToUnitGroupDataSet",
                            "value": {
                                "shortDescription": [
                                    {
                                        "value": "MJ"
                                    }
                                ],
                                "type": "unit group data set",
                                "refObjectId": "93a60a57-a3c8-11da-a746-0800200c9a66",
                                "uri": "../unitgroups/93a60a57-a3c8-11da-a746-0800200c9a66"
                            }
                        }
                    ]
                },
                "dataSetInternalID": 10
            },
            {
                "referenceToFlowDataSet": {
                    "shortDescription": [
                        {
                            "value": "Use of net fresh water (FW)",
                            "lang": "en"
                        },
                        {
                            "value": "Netto bruk av ferskvann (W)",
                            "lang": "no"
                        }
                    ],
                    "type": "flow data set",
                    "refObjectId": "3cf952c8-f3a4-461d-8c96-96456ca62246",
                    "version": "30.00.000"
                },
                "functionType": "General reminder flow",
                "exchangeDirection": "Input",
                "meanAmount": 0.0,
                "resultingAmount": 0.0,
                "minimumAmount": 0.0,
                "maximumAmount": 0.0,
                "uncertaintyDistributionType": "undefined",
                "relativeStandardDeviation95In": 0,
                "dataSourceType": "Primary",
                "dataDerivationTypeStatus": "Measured",
                "other": {
                    "anies": [
                        {
                            "value": "0.293202972792",
                            "module": "A1-A3"
                        },
                        {
                            "value": "0.000450766400",
                            "module": "A4"
                        },
                        {
                            "value": "0.000701033820",
                            "module": "A5"
                        },
                        {
                            "value": "0.000701033820",
                            "module": "C1"
                        },
                        {
                            "value": "0.000450766400",
                            "module": "C2"
                        },
                        {
                            "value": "0.000000000000",
                            "module": "C3"
                        },
                        {
                            "value": "0.000230417961",
                            "module": "C4"
                        },
                        {
                            "value": "-0.072501874060",
                            "module": "D"
                        },
                        {
                            "name": "referenceToUnitGroupDataSet",
                            "value": {
                                "shortDescription": [
                                    {
                                        "value": "m3"
                                    }
                                ],
                                "type": "unit group data set",
                                "refObjectId": "cd950537-0a98-4044-9ba7-9f9a68d0a504",
                                "uri": "../unitgroups/cd950537-0a98-4044-9ba7-9f9a68d0a504"
                            }
                        }
                    ]
                },
                "dataSetInternalID": 11
            },
            {
                "referenceToFlowDataSet": {
                    "shortDescription": [
                        {
                            "value": "Hazardous waste disposed (HWD)",
                            "lang": "en"
                        },
                        {
                            "value": "Avhendet farlig avfall (HW)",
                            "lang": "no"
                        }
                    ],
                    "type": "flow data set",
                    "refObjectId": "430f9e0f-59b2-46a0-8e0d-55e0e84948fc",
                    "version": "30.00.000"
                },
                "functionType": "General reminder flow",
                "exchangeDirection": "Output",
                "meanAmount": 0.0,
                "resultingAmount": 0.0,
                "minimumAmount": 0.0,
                "maximumAmount": 0.0,
                "uncertaintyDistributionType": "undefined",
                "relativeStandardDeviation95In": 0,
                "dataSourceType": "Primary",
                "dataDerivationTypeStatus": "Measured",
                "other": {
                    "anies": [
                        {
                            "value": "0.124759149909",
                            "module": "A1-A3"
                        },
                        {
                            "value": "0.000216739600",
                            "module": "A4"
                        },
                        {
                            "value": "0.000400949356",
                            "module": "A5"
                        },
                        {
                            "value": "0.000400949356",
                            "module": "C1"
                        },
                        {
                            "value": "0.000216739600",
                            "module": "C2"
                        },
                        {
                            "value": "0.000000000000",
                            "module": "C3"
                        },
                        {
                            "value": "0.000000000000",
                            "module": "C4"
                        },
                        {
                            "value": "-0.041285558271",
                            "module": "D"
                        },
                        {
                            "name": "referenceToUnitGroupDataSet",
                            "value": {
                                "shortDescription": [
                                    {
                                        "value": "kg"
                                    }
                                ],
                                "type": "unit group data set",
                                "refObjectId": "ad38d542-3fe9-439d-9b95-2f5f7752acaf",
                                "uri": "../unitgroups/ad38d542-3fe9-439d-9b95-2f5f7752acaf"
                            }
                        }
                    ]
                },
                "dataSetInternalID": 12
            },
            {
                "referenceToFlowDataSet": {
                    "shortDescription": [
                        {
                            "value": "Non hazardous waste dispose (NHWD)",
                            "lang": "en"
                        },
                        {
                            "value": "Avhendet ikke-farlig avfall (NHW)",
                            "lang": "no"
                        }
                    ],
                    "type": "flow data set",
                    "refObjectId": "b29ef66b-e286-4afa-949f-62f1a7b4d7fa",
                    "version": "30.00.000"
                },
                "functionType": "General reminder flow",
                "exchangeDirection": "Output",
                "meanAmount": 0.0,
                "resultingAmount": 0.0,
                "minimumAmount": 0.0,
                "maximumAmount": 0.0,
                "uncertaintyDistributionType": "undefined",
                "relativeStandardDeviation95In": 0,
                "dataSourceType": "Primary",
                "dataDerivationTypeStatus": "Measured",
                "other": {
                    "anies": [
                        {
                            "value": "9.558099737294",
                            "module": "A1-A3"
                        },
                        {
                            "value": "0.344310517600",
                            "module": "A4"
                        },
                        {
                            "value": "0.016127270914",
                            "module": "A5"
                        },
                        {
                            "value": "0.016127270914",
                            "module": "C1"
                        },
                        {
                            "value": "0.344310517600",
                            "module": "C2"
                        },
                        {
                            "value": "0.000000000000",
                            "module": "C3"
                        },
                        {
                            "value": "1.400000000000",
                            "module": "C4"
                        },
                        {
                            "value": "-1.236804956097",
                            "module": "D"
                        },
                        {
                            "name": "referenceToUnitGroupDataSet",
                            "value": {
                                "shortDescription": [
                                    {
                                        "value": "kg"
                                    }
                                ],
                                "type": "unit group data set",
                                "refObjectId": "ad38d542-3fe9-439d-9b95-2f5f7752acaf",
                                "uri": "../unitgroups/ad38d542-3fe9-439d-9b95-2f5f7752acaf"
                            }
                        }
                    ]
                },
                "dataSetInternalID": 13
            },
            {
                "referenceToFlowDataSet": {
                    "shortDescription": [
                        {
                            "value": "Radioactive waste disposed (RWD)",
                            "lang": "en"
                        },
                        {
                            "value": "Avhendet radioaktivt avfall (RW)",
                            "lang": "no"
                        }
                    ],
                    "type": "flow data set",
                    "refObjectId": "3449546e-52ad-4b39-b809-9fb77cea8ff6",
                    "version": "30.00.000"
                },
                "functionType": "General reminder flow",
                "exchangeDirection": "Output",
                "meanAmount": 0.0,
                "resultingAmount": 0.0,
                "minimumAmount": 0.0,
                "maximumAmount": 0.0,
                "uncertaintyDistributionType": "undefined",
                "relativeStandardDeviation95In": 0,
                "dataSourceType": "Primary",
                "dataDerivationTypeStatus": "Measured",
                "other": {
                    "anies": [
                        {
                            "value": "0.001164599637",
                            "module": "A1-A3"
                        },
                        {
                            "value": "0.000027048000",
                            "module": "A4"
                        },
                        {
                            "value": "0.000094580628",
                            "module": "A5"
                        },
                        {
                            "value": "0.000094580628",
                            "module": "C1"
                        },
                        {
                            "value": "0.000027048000",
                            "module": "C2"
                        },
                        {
                            "value": "0.000000000000",
                            "module": "C3"
                        },
                        {
                            "value": "0.000000000000",
                            "module": "C4"
                        },
                        {
                            "value": "-0.000159770475",
                            "module": "D"
                        },
                        {
                            "name": "referenceToUnitGroupDataSet",
                            "value": {
                                "shortDescription": [
                                    {
                                        "value": "kg"
                                    }
                                ],
                                "type": "unit group data set",
                                "refObjectId": "ad38d542-3fe9-439d-9b95-2f5f7752acaf",
                                "uri": "../unitgroups/ad38d542-3fe9-439d-9b95-2f5f7752acaf"
                            }
                        }
                    ]
                },
                "dataSetInternalID": 14
            },
            {
                "referenceToFlowDataSet": {
                    "shortDescription": [
                        {
                            "value": "Components for re-use (CRU)",
                            "lang": "en"
                        },
                        {
                            "value": "Komponenter for gjenbruk (CR)",
                            "lang": "no"
                        }
                    ],
                    "type": "flow data set",
                    "refObjectId": "a2b32f97-3fc7-4af2-b209-525bc6426f33",
                    "version": "30.00.000"
                },
                "functionType": "General reminder flow",
                "exchangeDirection": "Output",
                "meanAmount": 0.0,
                "resultingAmount": 0.0,
                "minimumAmount": 0.0,
                "maximumAmount": 0.0,
                "uncertaintyDistributionType": "undefined",
                "relativeStandardDeviation95In": 0,
                "dataSourceType": "Primary",
                "dataDerivationTypeStatus": "Measured",
                "other": {
                    "anies": [
                        {
                            "value": "0.000000000000",
                            "module": "A1-A3"
                        },
                        {
                            "value": "0.000000000000",
                            "module": "A4"
                        },
                        {
                            "value": "0.000000000000",
                            "module": "A5"
                        },
                        {
                            "value": "0.000000000000",
                            "module": "C1"
                        },
                        {
                            "value": "0.000000000000",
                            "module": "C2"
                        },
                        {
                            "value": "0.000000000000",
                            "module": "C3"
                        },
                        {
                            "value": "0.000000000000",
                            "module": "C4"
                        },
                        {
                            "value": "0.000000000000",
                            "module": "D"
                        },
                        {
                            "name": "referenceToUnitGroupDataSet",
                            "value": {
                                "shortDescription": [
                                    {
                                        "value": "kg"
                                    }
                                ],
                                "type": "unit group data set",
                                "refObjectId": "ad38d542-3fe9-439d-9b95-2f5f7752acaf",
                                "uri": "../unitgroups/ad38d542-3fe9-439d-9b95-2f5f7752acaf"
                            }
                        }
                    ]
                },
                "dataSetInternalID": 15
            },
            {
                "referenceToFlowDataSet": {
                    "shortDescription": [
                        {
                            "value": "Materials for recycling (MFR)",
                            "lang": "en"
                        },
                        {
                            "value": "Materialer for resirkulering (MR)",
                            "lang": "no"
                        }
                    ],
                    "type": "flow data set",
                    "refObjectId": "d7fe48a5-4103-49c8-9aae-b0b5dfdbd6ae",
                    "version": "30.00.000"
                },
                "functionType": "General reminder flow",
                "exchangeDirection": "Output",
                "meanAmount": 0.0,
                "resultingAmount": 0.0,
                "minimumAmount": 0.0,
                "maximumAmount": 0.0,
                "uncertaintyDistributionType": "undefined",
                "relativeStandardDeviation95In": 0,
                "dataSourceType": "Primary",
                "dataDerivationTypeStatus": "Measured",
                "other": {
                    "anies": [
                        {
                            "value": "1.585870051279",
                            "module": "A1-A3"
                        },
                        {
                            "value": "0.000000000000",
                            "module": "A4"
                        },
                        {
                            "value": "0.000000000000",
                            "module": "A5"
                        },
                        {
                            "value": "0.000000000000",
                            "module": "C1"
                        },
                        {
                            "value": "0.000000000000",
                            "module": "C2"
                        },
                        {
                            "value": "12.600000000000",
                            "module": "C3"
                        },
                        {
                            "value": "0.000000000000",
                            "module": "C4"
                        },
                        {
                            "value": "0.000000000000",
                            "module": "D"
                        },
                        {
                            "name": "referenceToUnitGroupDataSet",
                            "value": {
                                "shortDescription": [
                                    {
                                        "value": "kg"
                                    }
                                ],
                                "type": "unit group data set",
                                "refObjectId": "ad38d542-3fe9-439d-9b95-2f5f7752acaf",
                                "uri": "../unitgroups/ad38d542-3fe9-439d-9b95-2f5f7752acaf"
                            }
                        }
                    ]
                },
                "dataSetInternalID": 16
            },
            {
                "referenceToFlowDataSet": {
                    "shortDescription": [
                        {
                            "value": "Materials for energy recovery (MER)",
                            "lang": "en"
                        },
                        {
                            "value": "Materialer for energigjenvinning (MER)",
                            "lang": "no"
                        }
                    ],
                    "type": "flow data set",
                    "refObjectId": "59a9181c-3aaf-46ee-8b13-2b3723b6e447",
                    "version": "30.00.000"
                },
                "functionType": "General reminder flow",
                "exchangeDirection": "Output",
                "meanAmount": 0.0,
                "resultingAmount": 0.0,
                "minimumAmount": 0.0,
                "maximumAmount": 0.0,
                "uncertaintyDistributionType": "undefined",
                "relativeStandardDeviation95In": 0,
                "dataSourceType": "Primary",
                "dataDerivationTypeStatus": "Measured",
                "other": {
                    "anies": [
                        {
                            "value": "0.000021686611",
                            "module": "A1-A3"
                        },
                        {
                            "value": "0.000000000000",
                            "module": "A4"
                        },
                        {
                            "value": "0.000000000000",
                            "module": "A5"
                        },
                        {
                            "value": "0.000000000000",
                            "module": "C1"
                        },
                        {
                            "value": "0.000000000000",
                            "module": "C2"
                        },
                        {
                            "value": "0.000000000000",
                            "module": "C3"
                        },
                        {
                            "value": "0.000000000000",
                            "module": "C4"
                        },
                        {
                            "value": "0.000000000000",
                            "module": "D"
                        },
                        {
                            "name": "referenceToUnitGroupDataSet",
                            "value": {
                                "shortDescription": [
                                    {
                                        "value": "kg"
                                    }
                                ],
                                "type": "unit group data set",
                                "refObjectId": "ad38d542-3fe9-439d-9b95-2f5f7752acaf",
                                "uri": "../unitgroups/ad38d542-3fe9-439d-9b95-2f5f7752acaf"
                            }
                        }
                    ]
                },
                "dataSetInternalID": 17
            },
            {
                "referenceToFlowDataSet": {
                    "shortDescription": [
                        {
                            "value": "Exported electrical energy (EEE)",
                            "lang": "en"
                        },
                        {
                            "value": "Eksportert elektrisk energi(EEE)",
                            "lang": "no"
                        }
                    ],
                    "type": "flow data set",
                    "refObjectId": "4da0c987-2b76-40d6-9e9e-82a017aaaf29",
                    "version": "30.00.000"
                },
                "functionType": "General reminder flow",
                "exchangeDirection": "Output",
                "meanAmount": 0.0,
                "resultingAmount": 0.0,
                "minimumAmount": 0.0,
                "maximumAmount": 0.0,
                "uncertaintyDistributionType": "undefined",
                "relativeStandardDeviation95In": 0,
                "dataSourceType": "Primary",
                "dataDerivationTypeStatus": "Measured",
                "other": {
                    "anies": [
                        {
                            "value": "0.000000026562",
                            "module": "A1-A3"
                        },
                        {
                            "value": "0.000000000000",
                            "module": "A4"
                        },
                        {
                            "value": "0.000000000000",
                            "module": "A5"
                        },
                        {
                            "value": "0.000000000000",
                            "module": "C1"
                        },
                        {
                            "value": "0.000000000000",
                            "module": "C2"
                        },
                        {
                            "value": "0.000000000000",
                            "module": "C3"
                        },
                        {
                            "value": "0.000000000000",
                            "module": "C4"
                        },
                        {
                            "value": "0.000000000000",
                            "module": "D"
                        },
                        {
                            "name": "referenceToUnitGroupDataSet",
                            "value": {
                                "shortDescription": [
                                    {
                                        "value": "MJ"
                                    }
                                ],
                                "type": "unit group data set",
                                "refObjectId": "93a60a57-a3c8-11da-a746-0800200c9a66",
                                "uri": "../unitgroups/93a60a57-a3c8-11da-a746-0800200c9a66"
                            }
                        }
                    ]
                },
                "dataSetInternalID": 18
            },
            {
                "referenceToFlowDataSet": {
                    "shortDescription": [
                        {
                            "value": "Exported thermal energy (EET)",
                            "lang": "en"
                        },
                        {
                            "value": "Eksportert termisk energi (ETE)",
                            "lang": "no"
                        }
                    ],
                    "type": "flow data set",
                    "refObjectId": "98daf38a-7a79-46d3-9a37-2b7bd0955810",
                    "version": "30.00.000"
                },
                "functionType": "General reminder flow",
                "exchangeDirection": "Output",
                "meanAmount": 0.0,
                "resultingAmount": 0.0,
                "minimumAmount": 0.0,
                "maximumAmount": 0.0,
                "uncertaintyDistributionType": "undefined",
                "relativeStandardDeviation95In": 0,
                "dataSourceType": "Primary",
                "dataDerivationTypeStatus": "Measured",
                "other": {
                    "anies": [
                        {
                            "value": "0.000000401869",
                            "module": "A1-A3"
                        },
                        {
                            "value": "0.000000000000",
                            "module": "A4"
                        },
                        {
                            "value": "0.000000000000",
                            "module": "A5"
                        },
                        {
                            "value": "0.000000000000",
                            "module": "C1"
                        },
                        {
                            "value": "0.000000000000",
                            "module": "C2"
                        },
                        {
                            "value": "0.000000000000",
                            "module": "C3"
                        },
                        {
                            "value": "0.000000000000",
                            "module": "C4"
                        },
                        {
                            "value": "0.000000000000",
                            "module": "D"
                        },
                        {
                            "name": "referenceToUnitGroupDataSet",
                            "value": {
                                "shortDescription": [
                                    {
                                        "value": "MJ"
                                    }
                                ],
                                "type": "unit group data set",
                                "refObjectId": "93a60a57-a3c8-11da-a746-0800200c9a66",
                                "uri": "../unitgroups/93a60a57-a3c8-11da-a746-0800200c9a66"
                            }
                        }
                    ]
                },
                "dataSetInternalID": 19
            }
        ]
    },
    "LCIAResults": {
        "LCIAResult": [
            {
                "referenceToLCIAMethodDataSet": {
                    "shortDescription": [
                        {
                            "value": "Acidification potential, Accumulated Exceedance (AP)",
                            "lang": "en"
                        },
                        {
                            "value": "Forsurningspotensial for kilder p\u00e5 land og vann (AP)",
                            "lang": "no"
                        }
                    ],
                    "type": "LCIA method data set",
                    "refObjectId": "b5c611c6-def3-11e6-bf01-fe55135034f3",
                    "version": "00.01.000"
                },
                "meanAmount": 0.0,
                "uncertaintyDistributionType": "undefined",
                "relativeStandardDeviation95In": 0,
                "other": {
                    "anies": [
                        {
                            "value": "0.243636608038",
                            "module": "A1-A3"
                        },
                        {
                            "value": "0.000785260000",
                            "module": "A4"
                        },
                        {
                            "value": "0.010352886786",
                            "module": "A5"
                        },
                        {
                            "value": "0.010352886786",
                            "module": "C1"
                        },
                        {
                            "value": "0.000785260000",
                            "module": "C2"
                        },
                        {
                            "value": "0.000000000000",
                            "module": "C3"
                        },
                        {
                            "value": "0.000058506962",
                            "module": "C4"
                        },
                        {
                            "value": "-0.032524829534",
                            "module": "D"
                        },
                        {
                            "name": "referenceToUnitGroupDataSet",
                            "value": {
                                "shortDescription": [
                                    {
                                        "value": "mol H+ eqv."
                                    }
                                ],
                                "type": "unit group data set",
                                "refObjectId": "42e089ac-92bf-4bf2-8ca1-5fc40d18f2ed",
                                "uri": "../unitgroups/42e089ac-92bf-4bf2-8ca1-5fc40d18f2ed"
                            }
                        }
                    ]
                }
            },
            {
                "referenceToLCIAMethodDataSet": {
                    "shortDescription": [
                        {
                            "value": "Global Warming Potential - total (GWP-total)",
                            "lang": "en"
                        },
                        {
                            "value": "Globalt oppvarmingspotensial -totalt (GWPtotal)",
                            "lang": "no"
                        }
                    ],
                    "type": "LCIA method data set",
                    "refObjectId": "6a37f984-a4b3-458a-a20a-64418c145fa2",
                    "version": "00.02.000"
                },
                "meanAmount": 0.0,
                "uncertaintyDistributionType": "undefined",
                "relativeStandardDeviation95In": 0,
                "other": {
                    "anies": [
                        {
                            "value": "28.080406147473",
                            "module": "A1-A3"
                        },
                        {
                            "value": "0.244045743200",
                            "module": "A4"
                        },
                        {
                            "value": "0.989939442108",
                            "module": "A5"
                        },
                        {
                            "value": "0.989939442108",
                            "module": "C1"
                        },
                        {
                            "value": "0.244045743200",
                            "module": "C2"
                        },
                        {
                            "value": "0.000000000000",
                            "module": "C3"
                        },
                        {
                            "value": "0.006001093848",
                            "module": "C4"
                        },
                        {
                            "value": "-4.445215100312",
                            "module": "D"
                        },
                        {
                            "name": "referenceToUnitGroupDataSet",
                            "value": {
                                "shortDescription": [
                                    {
                                        "value": "kg CO2 eqv."
                                    }
                                ],
                                "type": "unit group data set",
                                "refObjectId": "1ebf3012-d0db-4de2-aefd-ef30cedb0be1",
                                "uri": "../unitgroups/1ebf3012-d0db-4de2-aefd-ef30cedb0be1"
                            }
                        }
                    ]
                }
            },
            {
                "referenceToLCIAMethodDataSet": {
                    "shortDescription": [
                        {
                            "value": "Global Warming Potential - biogenic (GWP-biogenic)",
                            "lang": "en"
                        },
                        {
                            "value": "Globalt oppvarmingspotensial - biogene kilder( GWP-biogenic)",
                            "lang": "no"
                        }
                    ],
                    "type": "LCIA method data set",
                    "refObjectId": "2356e1ab-0185-4db5-86e5-16de51c7485c",
                    "version": "00.02.000"
                },
                "meanAmount": 0.0,
                "uncertaintyDistributionType": "undefined",
                "relativeStandardDeviation95In": 0,
                "other": {
                    "anies": [
                        {
                            "value": "0.072852736517",
                            "module": "A1-A3"
                        },
                        {
                            "value": "0.000104462400",
                            "module": "A4"
                        },
                        {
                            "value": "0.000185538380",
                            "module": "A5"
                        },
                        {
                            "value": "0.000185538380",
                            "module": "C1"
                        },
                        {
                            "value": "0.000104462400",
                            "module": "C2"
                        },
                        {
                            "value": "0.000000000000",
                            "module": "C3"
                        },
                        {
                            "value": "0.000005098969",
                            "module": "C4"
                        },
                        {
                            "value": "-0.022105394876",
                            "module": "D"
                        },
                        {
                            "name": "referenceToUnitGroupDataSet",
                            "value": {
                                "shortDescription": [
                                    {
                                        "value": "kg CO2 eqv."
                                    }
                                ],
                                "type": "unit group data set",
                                "refObjectId": "1ebf3012-d0db-4de2-aefd-ef30cedb0be1",
                                "uri": "../unitgroups/1ebf3012-d0db-4de2-aefd-ef30cedb0be1"
                            }
                        }
                    ]
                }
            },
            {
                "referenceToLCIAMethodDataSet": {
                    "shortDescription": [
                        {
                            "value": "Global Warming Potential - fossil fuels (GWP-fossil)",
                            "lang": "en"
                        },
                        {
                            "value": "Globalt oppvarmingspotensial - fossile brensler (GWP-fossil)",
                            "lang": "no"
                        }
                    ],
                    "type": "LCIA method data set",
                    "refObjectId": "5f635281-343e-44fb-83df-1971b155e6b6",
                    "version": "00.01.000"
                },
                "meanAmount": 0.0,
                "uncertaintyDistributionType": "undefined",
                "relativeStandardDeviation95In": 0,
                "other": {
                    "anies": [
                        {
                            "value": "27.975491509842",
                            "module": "A1-A3"
                        },
                        {
                            "value": "0.243866977200",
                            "module": "A4"
                        },
                        {
                            "value": "0.989675903919",
                            "module": "A5"
                        },
                        {
                            "value": "0.989675903919",
                            "module": "C1"
                        },
                        {
                            "value": "0.243866977200",
                            "module": "C2"
                        },
                        {
                            "value": "0.000000000000",
                            "module": "C3"
                        },
                        {
                            "value": "0.005994819157",
                            "module": "C4"
                        },
                        {
                            "value": "-4.414909018821",
                            "module": "D"
                        },
                        {
                            "name": "referenceToUnitGroupDataSet",
                            "value": {
                                "shortDescription": [
                                    {
                                        "value": "kg CO2 eqv."
                                    }
                                ],
                                "type": "unit group data set",
                                "refObjectId": "1ebf3012-d0db-4de2-aefd-ef30cedb0be1",
                                "uri": "../unitgroups/1ebf3012-d0db-4de2-aefd-ef30cedb0be1"
                            }
                        }
                    ]
                }
            },
            {
                "referenceToLCIAMethodDataSet": {
                    "shortDescription": [
                        {
                            "value": "Global Warming Potential - land use and land use change (GWP-luluc)",
                            "lang": "en"
                        },
                        {
                            "value": "Globalt oppvarmingspotensial arealbruk endringer i bruk av arealer (GWP-luluc)",
                            "lang": "no"
                        }
                    ],
                    "type": "LCIA method data set",
                    "refObjectId": "4331bbdb-978a-490d-8707-eeb047f01a55",
                    "version": "00.02.000"
                },
                "meanAmount": 0.0,
                "uncertaintyDistributionType": "undefined",
                "relativeStandardDeviation95In": 0,
                "other": {
                    "anies": [
                        {
                            "value": "0.035083277096",
                            "module": "A1-A3"
                        },
                        {
                            "value": "0.000074300800",
                            "module": "A4"
                        },
                        {
                            "value": "0.000077999809",
                            "module": "A5"
                        },
                        {
                            "value": "0.000077999809",
                            "module": "C1"
                        },
                        {
                            "value": "0.000074300800",
                            "module": "C2"
                        },
                        {
                            "value": "0.000000000000",
                            "module": "C3"
                        },
                        {
                            "value": "0.000001175723",
                            "module": "C4"
                        },
                        {
                            "value": "-0.008200686615",
                            "module": "D"
                        },
                        {
                            "name": "referenceToUnitGroupDataSet",
                            "value": {
                                "shortDescription": [
                                    {
                                        "value": "kg CO2 eqv."
                                    }
                                ],
                                "type": "unit group data set",
                                "refObjectId": "1ebf3012-d0db-4de2-aefd-ef30cedb0be1",
                                "uri": "../unitgroups/1ebf3012-d0db-4de2-aefd-ef30cedb0be1"
                            }
                        }
                    ]
                }
            },
            {
                "referenceToLCIAMethodDataSet": {
                    "shortDescription": [
                        {
                            "value": "Potential Comparative Toxic Unit for ecosystems (ETP-fw)",
                            "lang": "en"
                        },
                        {
                            "value": "\u00d8kotoksisitet, ferskvann (ETP-fw)",
                            "lang": "no"
                        }
                    ],
                    "type": "LCIA method data set",
                    "refObjectId": "ee1082d1-b0f7-43ca-a1f0-21e2a4a74511",
                    "version": "00.01.000"
                },
                "meanAmount": 0.0,
                "uncertaintyDistributionType": "undefined",
                "relativeStandardDeviation95In": 0,
                "other": {
                    "anies": [
                        {
                            "value": "928.896820880096",
                            "module": "A1-A3"
                        },
                        {
                            "value": "2.896263305600",
                            "module": "A4"
                        },
                        {
                            "value": "7.443860836516",
                            "module": "A5"
                        },
                        {
                            "value": "7.443860836516",
                            "module": "C1"
                        },
                        {
                            "value": "2.896263305600",
                            "module": "C2"
                        },
                        {
                            "value": "0.000000000000",
                            "module": "C3"
                        },
                        {
                            "value": "0.095686047696",
                            "module": "C4"
                        },
                        {
                            "value": "-238.258901470825",
                            "module": "D"
                        },
                        {
                            "name": "referenceToUnitGroupDataSet",
                            "value": {
                                "shortDescription": [
                                    {
                                        "value": "CTUe"
                                    }
                                ],
                                "type": "unit group data set",
                                "refObjectId": "aa959ded-f1eb-4efb-9c5c-2d60be36b3e6",
                                "uri": "../unitgroups/aa959ded-f1eb-4efb-9c5c-2d60be36b3e6"
                            }
                        }
                    ]
                }
            },
            {
                "referenceToLCIAMethodDataSet": {
                    "shortDescription": [
                        {
                            "value": "Potential incidence of disease due to PM emissions (PM)",
                            "lang": "en"
                        },
                        {
                            "value": "Partikkelutslipp (PM)",
                            "lang": "no"
                        }
                    ],
                    "type": "LCIA method data set",
                    "refObjectId": "b5c602c6-def3-11e6-bf01-fe55135034f3",
                    "version": "00.01.000"
                },
                "meanAmount": 0.0,
                "uncertaintyDistributionType": "undefined",
                "relativeStandardDeviation95In": 0,
                "other": {
                    "anies": [
                        {
                            "value": "0.000002283463",
                            "module": "A1-A3"
                        },
                        {
                            "value": "0.000000022400",
                            "module": "A4"
                        },
                        {
                            "value": "0.000000273865",
                            "module": "A5"
                        },
                        {
                            "value": "0.000000273865",
                            "module": "C1"
                        },
                        {
                            "value": "0.000000022400",
                            "module": "C2"
                        },
                        {
                            "value": "0.000000000000",
                            "module": "C3"
                        },
                        {
                            "value": "0.000000001246",
                            "module": "C4"
                        },
                        {
                            "value": "-0.000000272537",
                            "module": "D"
                        },
                        {
                            "name": "referenceToUnitGroupDataSet",
                            "value": {
                                "shortDescription": [
                                    {
                                        "value": "disease incidence"
                                    }
                                ],
                                "type": "unit group data set",
                                "refObjectId": "3883559b-648f-4afc-8ba2-0bd24f3affa3",
                                "uri": "../unitgroups/3883559b-648f-4afc-8ba2-0bd24f3affa3"
                            }
                        }
                    ]
                }
            },
            {
                "referenceToLCIAMethodDataSet": {
                    "shortDescription": [
                        {
                            "value": "Eutrophication potential - marine (EP-marine)",
                            "lang": "en"
                        },
                        {
                            "value": "Overgj\u00f8dslingspotensial til hav (EP-marine), hav og jord",
                            "lang": "no"
                        }
                    ],
                    "type": "LCIA method data set",
                    "refObjectId": "b5c619fa-def3-11e6-bf01-fe55135034f3",
                    "version": "00.01.000"
                },
                "meanAmount": 0.0,
                "uncertaintyDistributionType": "undefined",
                "relativeStandardDeviation95In": 0,
                "other": {
                    "anies": [
                        {
                            "value": "0.054647042422",
                            "module": "A1-A3"
                        },
                        {
                            "value": "0.000171950800",
                            "module": "A4"
                        },
                        {
                            "value": "0.004569666792",
                            "module": "A5"
                        },
                        {
                            "value": "0.004569666792",
                            "module": "C1"
                        },
                        {
                            "value": "0.000171950800",
                            "module": "C2"
                        },
                        {
                            "value": "0.000000000000",
                            "module": "C3"
                        },
                        {
                            "value": "0.000021940065",
                            "module": "C4"
                        },
                        {
                            "value": "-0.007026579916",
                            "module": "D"
                        },
                        {
                            "name": "referenceToUnitGroupDataSet",
                            "value": {
                                "shortDescription": [
                                    {
                                        "value": "kg N eqv."
                                    }
                                ],
                                "type": "unit group data set",
                                "refObjectId": "d05bb823-ecdf-4686-8c40-bf1d9257859f",
                                "uri": "../unitgroups/d05bb823-ecdf-4686-8c40-bf1d9257859f"
                            }
                        }
                    ]
                }
            },
            {
                "referenceToLCIAMethodDataSet": {
                    "shortDescription": [
                        {
                            "value": "Eutrophication potential - freshwater (EP-freshwater)",
                            "lang": "en"
                        },
                        {
                            "value": "Overgj\u00f8dslingspotensial til ferskvann (EP-freshwater)",
                            "lang": "no"
                        }
                    ],
                    "type": "LCIA method data set",
                    "refObjectId": "b53ec18f-7377-4ad3-86eb-cc3f4f276b2b",
                    "version": "00.01.000"
                },
                "meanAmount": 0.0,
                "uncertaintyDistributionType": "undefined",
                "relativeStandardDeviation95In": 0,
                "other": {
                    "anies": [
                        {
                            "value": "0.001507832923",
                            "module": "A1-A3"
                        },
                        {
                            "value": "0.000001940400",
                            "module": "A4"
                        },
                        {
                            "value": "0.000003602929",
                            "module": "A5"
                        },
                        {
                            "value": "0.000003602929",
                            "module": "C1"
                        },
                        {
                            "value": "0.000001940400",
                            "module": "C2"
                        },
                        {
                            "value": "0.000000000000",
                            "module": "C3"
                        },
                        {
                            "value": "0.000000044745",
                            "module": "C4"
                        },
                        {
                            "value": "-0.000386676077",
                            "module": "D"
                        },
                        {
                            "name": "referenceToUnitGroupDataSet",
                            "value": {
                                "shortDescription": [
                                    {
                                        "value": "kg P eqv."
                                    }
                                ],
                                "type": "unit group data set",
                                "refObjectId": "0429039d-a61d-4590-ba67-aa4a20a810a1",
                                "uri": "../unitgroups/0429039d-a61d-4590-ba67-aa4a20a810a1"
                            }
                        }
                    ]
                }
            },
            {
                "referenceToLCIAMethodDataSet": {
                    "shortDescription": [
                        {
                            "value": "Eutrophication potential - terrestrial (EP-terrestrial)",
                            "lang": "en"
                        },
                        {
                            "value": "Overgj\u00f8dslingspotensial til jord (EP-terrestrial)",
                            "lang": "no"
                        }
                    ],
                    "type": "LCIA method data set",
                    "refObjectId": "b5c614d2-def3-11e6-bf01-fe55135034f3",
                    "version": "00.01.000"
                },
                "meanAmount": 0.0,
                "uncertaintyDistributionType": "undefined",
                "relativeStandardDeviation95In": 0,
                "other": {
                    "anies": [
                        {
                            "value": "0.601488949867",
                            "module": "A1-A3"
                        },
                        {
                            "value": "0.001917885200",
                            "module": "A4"
                        },
                        {
                            "value": "0.050139782180",
                            "module": "A5"
                        },
                        {
                            "value": "0.050139782180",
                            "module": "C1"
                        },
                        {
                            "value": "0.001917885200",
                            "module": "C2"
                        },
                        {
                            "value": "0.000000000000",
                            "module": "C3"
                        },
                        {
                            "value": "0.000241718915",
                            "module": "C4"
                        },
                        {
                            "value": "-0.076662169439",
                            "module": "D"
                        },
                        {
                            "name": "referenceToUnitGroupDataSet",
                            "value": {
                                "shortDescription": [
                                    {
                                        "value": "mol N eqv."
                                    }
                                ],
                                "type": "unit group data set",
                                "refObjectId": "71b4d617-0ec9-4d3f-b65e-e438940c2401",
                                "uri": "../unitgroups/71b4d617-0ec9-4d3f-b65e-e438940c2401"
                            }
                        }
                    ]
                }
            },
            {
                "referenceToLCIAMethodDataSet": {
                    "shortDescription": [
                        {
                            "value": "Potential Comparative Toxic Unit for humans - cancer effects (HTP-c)",
                            "lang": "en"
                        },
                        {
                            "value": "Toksisitet p\u00e5virkning p\u00e5 mennesker, kreft (HTP-c)",
                            "lang": "no"
                        }
                    ],
                    "type": "LCIA method data set",
                    "refObjectId": "2299222a-bbd8-474f-9d4f-4dd1f18aea7c",
                    "version": "00.01.000"
                },
                "meanAmount": 0.0,
                "uncertaintyDistributionType": "undefined",
                "relativeStandardDeviation95In": 0,
                "other": {
                    "anies": [
                        {
                            "value": "0.000000209599",
                            "module": "A1-A3"
                        },
                        {
                            "value": "0.000000000000",
                            "module": "A4"
                        },
                        {
                            "value": "0.000000000289",
                            "module": "A5"
                        },
                        {
                            "value": "0.000000000289",
                            "module": "C1"
                        },
                        {
                            "value": "0.000000000000",
                            "module": "C2"
                        },
                        {
                            "value": "0.000000000000",
                            "module": "C3"
                        },
                        {
                            "value": "0.000000000003",
                            "module": "C4"
                        },
                        {
                            "value": "-0.000000023272",
                            "module": "D"
                        },
                        {
                            "name": "referenceToUnitGroupDataSet",
                            "value": {
                                "shortDescription": [
                                    {
                                        "value": "CTUh"
                                    }
                                ],
                                "type": "unit group data set",
                                "refObjectId": "d4c9523e-2d7e-49fd-8469-998f547d3a70",
                                "uri": "../unitgroups/d4c9523e-2d7e-49fd-8469-998f547d3a70"
                            }
                        }
                    ]
                }
            },
            {
                "referenceToLCIAMethodDataSet": {
                    "shortDescription": [
                        {
                            "value": "Potential Comparative Toxic Unit for humans - non-cancer effects (HTP-nc)",
                            "lang": "en"
                        },
                        {
                            "value": "Toksisitet p\u00e5virkning p\u00e5 mennesker, andre effekter enn kreft (HTP-nc) ",
                            "lang": "no"
                        }
                    ],
                    "type": "LCIA method data set",
                    "refObjectId": "3af763a5-b7a1-48c9-9cee-1f223481fcef",
                    "version": "00.01.000"
                },
                "meanAmount": 0.0,
                "uncertaintyDistributionType": "undefined",
                "relativeStandardDeviation95In": 0,
                "other": {
                    "anies": [
                        {
                            "value": "0.000004121251",
                            "module": "A1-A3"
                        },
                        {
                            "value": "0.000000002800",
                            "module": "A4"
                        },
                        {
                            "value": "0.000000006842",
                            "module": "A5"
                        },
                        {
                            "value": "0.000000006842",
                            "module": "C1"
                        },
                        {
                            "value": "0.000000002800",
                            "module": "C2"
                        },
                        {
                            "value": "0.000000000000",
                            "module": "C3"
                        },
                        {
                            "value": "0.000000000056",
                            "module": "C4"
                        },
                        {
                            "value": "-0.000000121875",
                            "module": "D"
                        },
                        {
                            "name": "referenceToUnitGroupDataSet",
                            "value": {
                                "shortDescription": [
                                    {
                                        "value": "CTUh"
                                    }
                                ],
                                "type": "unit group data set",
                                "refObjectId": "d4c9523e-2d7e-49fd-8469-998f547d3a70",
                                "uri": "../unitgroups/d4c9523e-2d7e-49fd-8469-998f547d3a70"
                            }
                        }
                    ]
                }
            },
            {
                "referenceToLCIAMethodDataSet": {
                    "shortDescription": [
                        {
                            "value": "Potential Human exposure efficiency relative to U235 (IRP)",
                            "lang": "en"
                        },
                        {
                            "value": "Ioniserende str\u00e5ling, helseeffekt (IRP)",
                            "lang": "no"
                        }
                    ],
                    "type": "LCIA method data set",
                    "refObjectId": "b5c632be-def3-11e6-bf01-fe55135034f3",
                    "version": "00.01.000"
                },
                "meanAmount": 0.0,
                "uncertaintyDistributionType": "undefined",
                "relativeStandardDeviation95In": 0,
                "other": {
                    "anies": [
                        {
                            "value": "1.236650150305",
                            "module": "A1-A3"
                        },
                        {
                            "value": "0.017312562400",
                            "module": "A4"
                        },
                        {
                            "value": "0.058369774517",
                            "module": "A5"
                        },
                        {
                            "value": "0.058369774517",
                            "module": "C1"
                        },
                        {
                            "value": "0.017312562400",
                            "module": "C2"
                        },
                        {
                            "value": "0.000000000000",
                            "module": "C3"
                        },
                        {
                            "value": "0.000839625513",
                            "module": "C4"
                        },
                        {
                            "value": "-0.227304834062",
                            "module": "D"
                        },
                        {
                            "name": "referenceToUnitGroupDataSet",
                            "value": {
                                "shortDescription": [
                                    {
                                        "value": "kBq U235 eqv."
                                    }
                                ],
                                "type": "unit group data set",
                                "refObjectId": "456b05bf-1415-44a9-9993-02452f554c09",
                                "uri": "../unitgroups/456b05bf-1415-44a9-9993-02452f554c09"
                            }
                        }
                    ]
                }
            },
            {
                "referenceToLCIAMethodDataSet": {
                    "shortDescription": [
                        {
                            "value": "Potential Soil quality index (SQP)",
                            "lang": "en"
                        },
                        {
                            "value": "P\u00e5virkninger knyttet til arealbruksendringer / jordkvalitet (SQP)",
                            "lang": "no"
                        }
                    ],
                    "type": "LCIA method data set",
                    "refObjectId": "b2ad6890-c78d-11e6-9d9d-cec0c932ce01",
                    "version": "00.01.000"
                },
                "meanAmount": 0.0,
                "uncertaintyDistributionType": "undefined",
                "relativeStandardDeviation95In": 0,
                "other": {
                    "anies": [
                        {
                            "value": "98.147216002772",
                            "module": "A1-A3"
                        },
                        {
                            "value": "4.540830361200",
                            "module": "A4"
                        },
                        {
                            "value": "1.728579950491",
                            "module": "A5"
                        },
                        {
                            "value": "1.728579950491",
                            "module": "C1"
                        },
                        {
                            "value": "4.540830361200",
                            "module": "C2"
                        },
                        {
                            "value": "0.000000000000",
                            "module": "C3"
                        },
                        {
                            "value": "0.705181434240",
                            "module": "C4"
                        },
                        {
                            "value": "-16.242038434937",
                            "module": "D"
                        },
                        {
                            "name": "referenceToUnitGroupDataSet",
                            "value": {
                                "shortDescription": [
                                    {
                                        "value": "unitless"
                                    }
                                ],
                                "type": "unit group data set",
                                "refObjectId": "f130951c-e67f-4f7f-8dd4-665de3974e18",
                                "uri": "../unitgroups/f130951c-e67f-4f7f-8dd4-665de3974e18"
                            }
                        }
                    ]
                }
            },
            {
                "referenceToLCIAMethodDataSet": {
                    "shortDescription": [
                        {
                            "value": "Depletion potential of the stratospheric ozone layer (ODP)",
                            "lang": "en"
                        },
                        {
                            "value": "Potensial for nedbryting av stratosf\u00e6risk ozon (ODP)",
                            "lang": "no"
                        }
                    ],
                    "type": "LCIA method data set",
                    "refObjectId": "b5c629d6-def3-11e6-bf01-fe55135034f3",
                    "version": "00.01.000"
                },
                "meanAmount": 0.0,
                "uncertaintyDistributionType": "undefined",
                "relativeStandardDeviation95In": 0,
                "other": {
                    "anies": [
                        {
                            "value": "0.000002350455",
                            "module": "A1-A3"
                        },
                        {
                            "value": "0.000000058800",
                            "module": "A4"
                        },
                        {
                            "value": "0.000000213735",
                            "module": "A5"
                        },
                        {
                            "value": "0.000000213735",
                            "module": "C1"
                        },
                        {
                            "value": "0.000000058800",
                            "module": "C2"
                        },
                        {
                            "value": "0.000000000000",
                            "module": "C3"
                        },
                        {
                            "value": "0.000000002919",
                            "module": "C4"
                        },
                        {
                            "value": "-0.000000238798",
                            "module": "D"
                        },
                        {
                            "name": "referenceToUnitGroupDataSet",
                            "value": {
                                "shortDescription": [
                                    {
                                        "value": "kg CFC 11 eqv."
                                    }
                                ],
                                "type": "unit group data set",
                                "refObjectId": "d9e957c9-7309-4474-bf3a-7777df6c4e5b",
                                "uri": "../unitgroups/d9e957c9-7309-4474-bf3a-7777df6c4e5b"
                            }
                        }
                    ]
                }
            },
            {
                "referenceToLCIAMethodDataSet": {
                    "shortDescription": [
                        {
                            "value": "Photochemical Ozone Creation Potential (POCP)",
                            "lang": "en"
                        },
                        {
                            "value": "Potensial for fotokjemisk oksidantdanning (POCP)",
                            "lang": "no"
                        }
                    ],
                    "type": "LCIA method data set",
                    "refObjectId": "b5c610fe-def3-11e6-bf01-fe55135034f3",
                    "version": "00.01.000"
                },
                "meanAmount": 0.0,
                "uncertaintyDistributionType": "undefined",
                "relativeStandardDeviation95In": 0,
                "other": {
                    "anies": [
                        {
                            "value": "0.190992264380",
                            "module": "A1-A3"
                        },
                        {
                            "value": "0.000753135600",
                            "module": "A4"
                        },
                        {
                            "value": "0.013785959350",
                            "module": "A5"
                        },
                        {
                            "value": "0.013785959350",
                            "module": "C1"
                        },
                        {
                            "value": "0.000753135600",
                            "module": "C2"
                        },
                        {
                            "value": "0.000000000000",
                            "module": "C3"
                        },
                        {
                            "value": "0.000069156758",
                            "module": "C4"
                        },
                        {
                            "value": "-0.024592995863",
                            "module": "D"
                        },
                        {
                            "name": "referenceToUnitGroupDataSet",
                            "value": {
                                "shortDescription": [
                                    {
                                        "value": "kg NMVOC eqv."
                                    }
                                ],
                                "type": "unit group data set",
                                "refObjectId": "d27c25f8-fbc1-44c6-b47b-4adbae4199c6",
                                "uri": "../unitgroups/d27c25f8-fbc1-44c6-b47b-4adbae4199c6"
                            }
                        }
                    ]
                }
            },
            {
                "referenceToLCIAMethodDataSet": {
                    "shortDescription": [
                        {
                            "value": "Abiotic depletion potential - fossil resources (ADPF)",
                            "lang": "en"
                        },
                        {
                            "value": "Abiotisk utarmingspotensial for fossile ressurser, fosile brensler (ADP-fossil)",
                            "lang": "no"
                        }
                    ],
                    "type": "LCIA method data set",
                    "refObjectId": "b2ad6110-c78d-11e6-9d9d-cec0c932ce01",
                    "version": "00.01.000"
                },
                "meanAmount": 0.0,
                "uncertaintyDistributionType": "undefined",
                "relativeStandardDeviation95In": 0,
                "other": {
                    "anies": [
                        {
                            "value": "342.979339625164",
                            "module": "A1-A3"
                        },
                        {
                            "value": "3.961368871600",
                            "module": "A4"
                        },
                        {
                            "value": "13.620976974868",
                            "module": "A5"
                        },
                        {
                            "value": "13.620976974868",
                            "module": "C1"
                        },
                        {
                            "value": "3.961368871600",
                            "module": "C2"
                        },
                        {
                            "value": "0.000000000000",
                            "module": "C3"
                        },
                        {
                            "value": "0.193442793604",
                            "module": "C4"
                        },
                        {
                            "value": "-50.909129117559",
                            "module": "D"
                        },
                        {
                            "name": "referenceToUnitGroupDataSet",
                            "value": {
                                "shortDescription": [
                                    {
                                        "value": "MJ"
                                    }
                                ],
                                "type": "unit group data set",
                                "refObjectId": "93a60a57-a3c8-11da-a746-0800200c9a66",
                                "uri": "../unitgroups/93a60a57-a3c8-11da-a746-0800200c9a66"
                            }
                        }
                    ]
                }
            },
            {
                "referenceToLCIAMethodDataSet": {
                    "shortDescription": [
                        {
                            "value": "Abiotic depletion potential - non-fossil resources (ADPE)",
                            "lang": "en"
                        },
                        {
                            "value": "Abiotisk utarmingspotensial for ikke-fossile ressurser, mineraler (ADP-elements)",
                            "lang": "no"
                        }
                    ],
                    "type": "LCIA method data set",
                    "refObjectId": "b2ad6494-c78d-11e6-9d9d-cec0c932ce01",
                    "version": "00.01.000"
                },
                "meanAmount": 0.0,
                "uncertaintyDistributionType": "undefined",
                "relativeStandardDeviation95In": 0,
                "other": {
                    "anies": [
                        {
                            "value": "0.065270861332",
                            "module": "A1-A3"
                        },
                        {
                            "value": "0.000004345600",
                            "module": "A4"
                        },
                        {
                            "value": "0.000001518611",
                            "module": "A5"
                        },
                        {
                            "value": "0.000001518611",
                            "module": "C1"
                        },
                        {
                            "value": "0.000004345600",
                            "module": "C2"
                        },
                        {
                            "value": "0.000000000000",
                            "module": "C3"
                        },
                        {
                            "value": "0.000000053054",
                            "module": "C4"
                        },
                        {
                            "value": "-0.055400974856",
                            "module": "D"
                        },
                        {
                            "name": "referenceToUnitGroupDataSet",
                            "value": {
                                "shortDescription": [
                                    {
                                        "value": "kg Sb-eqv."
                                    }
                                ],
                                "type": "unit group data set",
                                "refObjectId": "54ccd2d9-a32a-4fc2-923d-f2c8c93e89d4",
                                "uri": "../unitgroups/54ccd2d9-a32a-4fc2-923d-f2c8c93e89d4"
                            }
                        }
                    ]
                }
            },
            {
                "referenceToLCIAMethodDataSet": {
                    "shortDescription": [
                        {
                            "value": "Water (user) deprivation potential (WDP)",
                            "lang": "en"
                        },
                        {
                            "value": "Utarmingspotensial for vannressurser (WDP)",
                            "lang": "no"
                        }
                    ],
                    "type": "LCIA method data set",
                    "refObjectId": "b2ad66ce-c78d-11e6-9d9d-cec0c932ce01",
                    "version": "00.01.000"
                },
                "meanAmount": 0.0,
                "uncertaintyDistributionType": "undefined",
                "relativeStandardDeviation95In": 0,
                "other": {
                    "anies": [
                        {
                            "value": "110.911852082507",
                            "module": "A1-A3"
                        },
                        {
                            "value": "3.037081846400",
                            "module": "A4"
                        },
                        {
                            "value": "2.893820187134",
                            "module": "A5"
                        },
                        {
                            "value": "2.893820187134",
                            "module": "C1"
                        },
                        {
                            "value": "3.037081846400",
                            "module": "C2"
                        },
                        {
                            "value": "0.000000000000",
                            "module": "C3"
                        },
                        {
                            "value": "0.407228422053",
                            "module": "C4"
                        },
                        {
                            "value": "36.701029429925",
                            "module": "D"
                        },
                        {
                            "name": "referenceToUnitGroupDataSet",
                            "value": {
                                "shortDescription": [
                                    {
                                        "value": "m3 world eqv."
                                    }
                                ],
                                "type": "unit group data set",
                                "refObjectId": "6ae2df01-888e-46c8-b17d-49fa3869b476",
                                "uri": "../unitgroups/6ae2df01-888e-46c8-b17d-49fa3869b476"
                            }
                        }
                    ]
                }
            },
            {
                "referenceToLCIAMethodDataSet": {
                    "shortDescription": [
                        {
                            "value": "Global warming potential except emissions and uptake of biogenic carbon (GWP-IOBC/GHG)",
                            "lang": "en"
                        },
                        {
                            "value": "Globalt oppvarmingspotensial beregnet etter prinsippet om umiddelbar oksidasjon (GWP-IOBC)",
                            "lang": "no"
                        }
                    ],
                    "type": "LCIA method data set",
                    "refObjectId": "fb774615-0575-45de-9a89-1ded92f19770",
                    "version": "00.01.000"
                },
                "meanAmount": 0.0,
                "uncertaintyDistributionType": "undefined",
                "relativeStandardDeviation95In": 0,
                "other": {
                    "anies": [
                        {
                            "value": "28.052241860294",
                            "module": "A1-A3"
                        },
                        {
                            "value": "0.244038186000",
                            "module": "A4"
                        },
                        {
                            "value": "0.989926013606",
                            "module": "A5"
                        },
                        {
                            "value": "0.989926013606",
                            "module": "C1"
                        },
                        {
                            "value": "0.244038186000",
                            "module": "C2"
                        },
                        {
                            "value": "0.000000000000",
                            "module": "C3"
                        },
                        {
                            "value": "0.006001093848",
                            "module": "C4"
                        },
                        {
                            "value": "-5.571260459521",
                            "module": "D"
                        },
                        {
                            "name": "referenceToUnitGroupDataSet",
                            "value": {
                                "shortDescription": [
                                    {
                                        "value": "kg CO2 eqv."
                                    }
                                ],
                                "type": "unit group data set",
                                "refObjectId": "1ebf3012-d0db-4de2-aefd-ef30cedb0be1",
                                "uri": "../unitgroups/1ebf3012-d0db-4de2-aefd-ef30cedb0be1"
                            }
                        }
                    ]
                }
            }
        ]
    },
    "otherAttributes": {
        "{http://www.indata.network/EPD/2019}epd-version": "1.2"
    },
    "version": "1.1"
}